cleanq/set: working on the weak conditions, converting the fun to definitions
Signed-off-by: Reto Achermann <reto.achermann@inf.ethz.ch>

CleanQ/CleanQ_SetModel.thy
@@ -24,13 +24,12 @@ imports
   Main
   "../Simpl/Simpl" 
   "../Complx/OG_Hoare"
-(*  "../Complx/OG_Syntax" *)
 begin
 (*>*)
 
+
 text \<open>
-  We now define the model state, its invariants and state transitions. Followed by proofs 
-  using Owicki-Gries (OG)
+  We now define the model state, its invariants and state transitions. 
 \<close>
 
 (* ==================================================================================== *)
@@ -67,7 +66,6 @@ text \<open>
 (* Define some global variables to make Simpl/Complex proofs work *)
 record 'g CleanQ_Set_State_vars = 
   SetRB_'  :: "nat CleanQ_Set_State"
-  B_'   ::  nat
 (*>*)
   
 
@@ -94,7 +92,7 @@ text \<open>
   Recall, the actual representation of buffer elements is undefined.
 \<close>
 
-fun I1 :: "'a CleanQ_Set_State \<Rightarrow> 'a set \<Rightarrow> bool"
+definition I1 :: "'a CleanQ_Set_State \<Rightarrow> 'a set \<Rightarrow> bool"
   where "I1 rb K \<longleftrightarrow> ((SX rb) \<union> (SY rb) \<union> (TXY rb) \<union> (TYX rb)) = K"
 
 
@@ -110,7 +108,7 @@ text \<open>
   for the state with two agents.
 \<close>
 
-fun I2 :: "'a CleanQ_Set_State \<Rightarrow> bool"
+definition I2 :: "'a CleanQ_Set_State \<Rightarrow> bool"
   where "I2 rb \<longleftrightarrow> SX rb \<inter> SY rb = {} \<and> SX rb \<inter> TXY rb = {} \<and> SX rb \<inter> TYX rb = {} \<and>
                    SY rb \<inter> TXY rb = {} \<and> SY rb \<inter> TYX rb = {} \<and> TXY rb \<inter> TYX rb = {}"
 
@@ -124,8 +122,12 @@ text \<open>
   predicate \verb+CleanQ_Set_Invariants+.
 \<close>
 
-fun CleanQ_Set_Invariants :: "'a set \<Rightarrow> 'a CleanQ_Set_State \<Rightarrow> bool"
+definition CleanQ_Set_Invariants :: "'a set \<Rightarrow> 'a CleanQ_Set_State \<Rightarrow> bool"
   where "CleanQ_Set_Invariants K rb \<longleftrightarrow> I1 rb K \<and> I2 rb"
+
+
+lemmas CleanQ_Set_Invariants_simp = CleanQ_Set_Invariants_def I1_def I2_def
+  
 
 
 (* ==================================================================================== *)
@@ -180,244 +182,25 @@ text \<open>
 \<close>
 
 lemma CleanQ_Set_enq_x_I1 :
-  assumes I1_holds: "I1 rb K"  and  X_owned: "b \<in> SX rb" 
-    shows "I1 (CleanQ_Set_enq_x b rb) K"
-  unfolding CleanQ_Set_enq_x_def 
-  using I1_holds X_owned by auto
+assumes I1_holds: "I1 rb K"  and  X_owned: "b \<in> SX rb" 
+  shows "I1 (CleanQ_Set_enq_x b rb) K"
+  using I1_holds X_owned unfolding CleanQ_Set_enq_x_def I1_def by auto
 
 lemma CleanQ_Set_enq_y_I1 :
-  assumes I1_holds: "I1 rb K"  and  X_owned: "b \<in> SY rb"
-    shows "I1 (CleanQ_Set_enq_y b rb) K"
-  unfolding CleanQ_Set_enq_y_def 
-  using I1_holds X_owned by auto
+assumes I1_holds: "I1 rb K"  and  X_owned: "b \<in> SY rb"
+  shows "I1 (CleanQ_Set_enq_y b rb) K"
+  using I1_holds X_owned unfolding CleanQ_Set_enq_y_def I1_def by auto
 
 lemma CleanQ_Set_enq_x_I2 :
-  assumes I2_holds: "I2 rb"  and  X_owned: "b \<in> SX rb"
-    shows "I2 (CleanQ_Set_enq_x b rb)"
-  unfolding CleanQ_Set_enq_x_def
-  using I2_holds X_owned by auto
+assumes I2_holds: "I2 rb"  and  X_owned: "b \<in> SX rb"
+  shows "I2 (CleanQ_Set_enq_x b rb)"
+  using I2_holds X_owned unfolding CleanQ_Set_enq_x_def I2_def  by auto
 
 lemma CleanQ_Set_enq_y_I2 :
-  assumes  I2_holds: "I2 rb"  and  X_owned: "b \<in> SY rb"
-    shows "I2 (CleanQ_Set_enq_y b rb)"
-  unfolding CleanQ_Set_enq_y_def
-  using I2_holds X_owned by auto
+assumes  I2_holds: "I2 rb"  and  X_owned: "b \<in> SY rb"
+  shows "I2 (CleanQ_Set_enq_y b rb)"
+  using I2_holds X_owned unfolding CleanQ_Set_enq_y_def I2_def by auto
 
-
-text \<open>The frame condition as we currently have it can be defined as shown below. The essence of
-      it is that no set changes which is not specifically defined to change.\<close>
-fun frame_strong ::
-  "'a \<times> 'b \<times> 'c \<times> 'd \<Rightarrow>'a \<times> 'b \<times> 'c \<times> 'd \<Rightarrow> bool"
-  where "frame_strong (A',B',C',D') (A,B,C,D) \<longleftrightarrow> A' = A \<and> B' = B \<and> C' = C \<and> D' = D"
-
-
-text \<open>
-  For the concurrent case, we can not assume that the sets we do not explicitly modify by an operation
-  do not change and for this we have to weaken the frame condition that e.g. when enqueueing 
-  from X the sets TXY, SY and TYX might change through actions of Y.
-\<close>
-
-text \<open>@{term D} is in its initial state, but elements may move from @{term A} to @{term B}
-  and from @{term B} to @{term C}.\<close>
-fun frame_weak ::
-  "'a set \<times> 'a set \<times> 'a set \<times> 'a set \<Rightarrow> 'a set \<times> 'a set \<times> 'a set \<times> 'a set \<Rightarrow> bool"
-  where "frame_weak (A',B',C',D') (A,B,C,D) \<longleftrightarrow> (\<exists>\<Delta>AB \<Delta>BC.
-    A' = \<Delta>AB \<union> A \<and>
-    B' \<union> \<Delta>AB = \<Delta>BC \<union> B \<and>
-    C' \<union> \<Delta>BC = C \<and>
-    A \<inter> \<Delta>AB = {} \<and>
-    A \<inter> \<Delta>BC = {} \<and>
-    B \<inter> \<Delta>BC = {})
-  \<and> D' = D"
-
-text \<open>
-  As a first step we have to show that the strong frame condition implies the weak one.
-\<close>
-
-lemma frame_s_w:
-  "frame_strong (A',B',C',D') (A,B,C,D) \<Longrightarrow> frame_weak (A',B',C',D') (A,B,C,D)"
-  unfolding frame_strong.simps frame_weak.simps by(blast)
-
-text \<open>The weak frame condition for an enqueue from @{term D} into @{term A} preserves
-  invariant 1.\<close>
-
-lemma CleanQ_Set_enq_x_I1_weak:
-  fixes st st' K b
-  assumes I: "CleanQ_Set_Invariants K st'"
-      and rb: "st = CleanQ_Set_enq b st'"
-      and frame: "frame_weak (TXY st' \<union> {b},SY st', TYX st', SX st' - {b}) (TXY st, SY st, TYX st, SX st)"
-      and owns: "b \<in> SX st'"
-    shows "I1 st K"
-proof -
-  from frame obtain \<Delta>AB \<Delta>BC where
-    fA: "(TXY st' \<union> {b}) = \<Delta>AB \<union> TXY st" and
-    fB: "SY st' \<union> \<Delta>AB = \<Delta>BC \<union> SY st" and
-    fC: "TYX st' \<union> \<Delta>BC = TYX st" and
-    fD: "SX st' - {b} = SX st"
-    by(auto)
-
-  from fC have "TYX st = TYX st' \<union> \<Delta>BC" by(simp)
-  hence "SY st \<union> TYX st = (SY st \<union> \<Delta>BC) \<union> TYX st'" by(simp add:ac_simps)
-  with fB have "SY st \<union> TYX st = (SY st' \<union> \<Delta>AB) \<union> TYX st'" by(simp add:ac_simps)
-  hence "TXY st \<union> SY st \<union> TYX st = (TXY st \<union> \<Delta>AB) \<union> SY st' \<union> TYX st'"by blast
-  with fA have "TXY st \<union> SY st \<union> TYX st = (TXY st' \<union> {b}) \<union> SY st' \<union> TYX st'" by(simp add:ac_simps)
-  with fD have "TXY st \<union> SY st \<union> TYX st \<union> SX st = (TXY st' \<union> {b}) \<union> SY st' \<union> TYX st' \<union> (SX st' - {b})" by(simp)
-  also from owns have "... = TXY st' \<union> SY st' \<union> TYX st' \<union> SX st'" by(auto)
-  also from I have "... = K" by auto
-  finally show ?thesis by auto
-qed
-
-lemma CleanQ_Set_enq_y_I1_weak:
-  fixes st st' K b
-  assumes I: "CleanQ_Set_Invariants K st'"
-      and rb: "st = CleanQ_Set_enq b st'"
-      and frame: "frame_weak (TYX st' \<union> {b},SX st', TXY st', SY st' - {b}) (TYX st, SX st, TXY st, SY st)"
-      and owns: "b \<in> SY st'"
-    shows "I1 st K"
-proof -
-  from frame obtain \<Delta>AB \<Delta>BC where
-    fA: "(TYX st' \<union> {b}) = \<Delta>AB \<union> TYX st" and
-    fB: "SX st' \<union> \<Delta>AB = \<Delta>BC \<union> SX st" and
-    fC: "TXY st' \<union> \<Delta>BC = TXY st" and
-    fD: "SY st' - {b} = SY st"
-    by(auto)
-
-  from fC have "TXY st = TXY st' \<union> \<Delta>BC" by(simp)
-  hence "SX st \<union> TXY st = (SX st \<union> \<Delta>BC) \<union> TXY st'" by(simp add:ac_simps)
-  with fB have "SX st \<union> TXY st = (SX st' \<union> \<Delta>AB) \<union> TXY st'" by(simp add:ac_simps)
-  hence "TYX st \<union> SX st \<union> TXY st = (TYX st \<union> \<Delta>AB) \<union> SX st' \<union> TXY st'"by blast
-  with fA have "TYX st \<union> SX st \<union> TXY st = (TYX st' \<union> {b}) \<union> SX st' \<union> TXY st'" by(simp add:ac_simps)
-  with fD have "TYX st \<union> SX st \<union> TXY st \<union> SY st = (TYX st' \<union> {b}) \<union> SX st' \<union> TXY st' \<union> (SY st' - {b})" by(simp)
-  also from owns have "... = TYX st' \<union> SX st' \<union> TXY st' \<union> SY st'" by(auto)
-  also from I have "... = K" by auto
-  finally show ?thesis by auto
-qed
-
-lemma CleanQ_Set_enq_x_I2_weak:
-  fixes st st' K b
-  assumes I: "CleanQ_Set_Invariants K st'"
-      and rb: "st = CleanQ_Set_enq b st'"
-      and frame: "frame_weak (TXY st' \<union> {b},SY st', TYX st', SX st' - {b}) (TXY st, SY st, TYX st, SX st)"
-      and owns: "b \<in> SX st'"
-    shows "I2 st"
-proof(unfold I2.simps, intro conjI)
-  from frame obtain \<Delta>AB \<Delta>BC where
-    fA: "(TXY st' \<union> {b}) = \<Delta>AB \<union> TXY st" and
-    fB: "SY st' \<union> \<Delta>AB = \<Delta>BC \<union> SY st" and
-    fC: "TYX st' \<union> \<Delta>BC = TYX st" and
-    fD: "SX st' - {b} = SX st" and
-    dAB: "TXY st \<inter> \<Delta>AB = {}" and
-    dAC: "TXY st \<inter> \<Delta>BC = {}" and
-    dBC: "SY st \<inter> \<Delta>BC = {}"
-    by auto
-
-  from fA have ss_\<Delta>AB: "\<Delta>AB \<subseteq> TXY st' \<union> {b}" by(auto)
-  with fB have ss_\<Delta>BC: "\<Delta>BC \<subseteq> TXY st' \<union> SY st' \<union> {b}" by(auto)
-
-  from fA have ss_A: "TXY st \<subseteq> TXY st' \<union> {b}" by(auto)
-  from fB ss_\<Delta>AB have ss_B: "SY st \<subseteq> TXY st' \<union> SY st' \<union> {b}" by(auto)
-  from fC ss_\<Delta>BC have ss_C: "TYX st \<subseteq> TXY st' \<union> SY st' \<union> TYX st' \<union> {b}" by(auto)
-
-  from I ss_A show "SX st \<inter> TXY st = {}" by(unfold fD[symmetric], auto)
-  from I ss_B show "SX st \<inter> SY st = {}" by(unfold fD[symmetric], auto)
-  from I ss_C show "SX st \<inter> TYX st = {}" by(unfold fD[symmetric], auto)
-
-  from fC have "SY st \<inter> TYX st = SY st \<inter> (TYX st' \<union> \<Delta>BC)" by(simp)
-  also have "... = (SY st \<inter> TYX st') \<union> (SY st \<inter> \<Delta>BC)" by(auto)
-  also {
-    from ss_B have "SY st \<inter> TYX st' \<subseteq> (TXY st' \<union> SY st' \<union> {b}) \<inter> TYX st'" by(auto)
-    also from I owns have "... = {}" by(auto)
-    finally have "(SY st \<inter> TYX st') \<union> (SY st \<inter> \<Delta>BC) = SY st \<inter> \<Delta>BC" by(simp)
-  }
-  txt \<open>@{term "SY st \<inter> \<Delta>BC = {}"} is essential\<close>
-  finally have "SY st \<inter> TYX st = SY st \<inter> \<Delta>BC" .
-  with dBC show "SY st \<inter> TYX st = {}" by(simp)
-
-  from fC have "TXY st \<inter> TYX st = TXY st \<inter> (TYX st' \<union> \<Delta>BC)" by(simp)
-  also have "... = (TXY st \<inter> TYX st') \<union> (TXY st \<inter> \<Delta>BC)" by(auto)
-  also {
-    from ss_A have "TXY st \<inter> TYX st' \<subseteq> (TXY st' \<union> {b}) \<inter> TYX st'" by(auto)
-    also from I owns have "... = {}" by(auto)
-    finally have "(TXY st \<inter> TYX st') \<union> (TXY st \<inter> \<Delta>BC) = TXY st \<inter> \<Delta>BC" by(simp)
-  }
-  txt \<open>@{term "TXY st \<inter> \<Delta>BC = {}"} is essential\<close>
-  finally have "TXY st \<inter> TYX st = TXY st \<inter> \<Delta>BC" .
-  with dAC show "TXY st \<inter> TYX st = {}" by(simp)
-
-  from fB have "TXY st \<inter> (\<Delta>BC \<union> SY st) = TXY st \<inter> (SY st' \<union> \<Delta>AB)" by(simp)
-  also have "... = (TXY st \<inter> SY st') \<union> (TXY st \<inter> \<Delta>AB)" by(auto)
-  also {
-    from ss_A have "TXY st \<inter> SY st' \<subseteq> (TXY st' \<union> {b}) \<inter> SY st'" by(auto)
-    also from I owns have "... = {}" by(auto)
-    finally have "(TXY st \<inter> SY st') \<union> (TXY st \<inter> \<Delta>AB) = TXY st \<inter> \<Delta>AB" by(simp)
-  }
-  txt \<open>@{term "TXY st \<inter> \<Delta>AB = {}"} is essential, given @{term "TXY st \<inter> \<Delta>BC = {}"}.\<close>
-  finally have "TXY st \<inter> (\<Delta>BC \<union> SY st) = TXY st \<inter> \<Delta>AB" .
-  with dAB show "SY st \<inter> TXY st = {}" by auto
-qed
-
-lemma CleanQ_Set_enq_y_I2_weak:
-  fixes st st' K b
-  assumes I: "CleanQ_Set_Invariants K st'"
-      and rb: "st = CleanQ_Set_enq b st'"
-      and frame: "frame_weak (TYX st' \<union> {b},SX st', TXY st', SY st' - {b}) (TYX st, SX st, TXY st, SY st)"
-      and owns: "b \<in> SY st'"
-    shows "I2 st"
-proof(unfold I2.simps, intro conjI)
-  from frame obtain \<Delta>AB \<Delta>BC where
-    fA: "(TYX st' \<union> {b}) = \<Delta>AB \<union> TYX st" and
-    fB: "SX st' \<union> \<Delta>AB = \<Delta>BC \<union> SX st" and
-    fC: "TXY st' \<union> \<Delta>BC = TXY st" and
-    fD: "SY st' - {b} = SY st" and
-    dAB: "TYX st \<inter> \<Delta>AB = {}" and
-    dAC: "TYX st \<inter> \<Delta>BC = {}" and
-    dBC: "SX st \<inter> \<Delta>BC = {}"
-    by auto
-
-  from fA have ss_\<Delta>AB: "\<Delta>AB \<subseteq> TYX st' \<union> {b}" by(auto)
-  with fB have ss_\<Delta>BC: "\<Delta>BC \<subseteq> TYX st' \<union> SX st' \<union> {b}" by(auto)
-
-  from fA have ss_A: "TYX st \<subseteq> TYX st' \<union> {b}" by(auto)
-  from fB ss_\<Delta>AB have ss_B: "SX st \<subseteq> TYX st' \<union> SX st' \<union> {b}" by(auto)
-  from fC ss_\<Delta>BC have ss_C: "TXY st \<subseteq> TYX st' \<union> SX st' \<union> TXY st' \<union> {b}" by(auto)
-
-  from I ss_A show "SY st \<inter> TYX st = {}" by(unfold fD[symmetric], auto)
-  from I ss_B show "SX st \<inter> SY st = {}" by(unfold fD[symmetric], auto)
-  from I ss_C show "SY st \<inter> TXY st = {}" by(unfold fD[symmetric], auto)
-
-  from fC have "SX st \<inter> TXY st = SX st \<inter> (TXY st' \<union> \<Delta>BC)" by(simp)
-  also have "... = (SX st \<inter> TXY st') \<union> (SX st \<inter> \<Delta>BC)" by(auto)
-  also {
-    from ss_B have "SX st \<inter> TXY st' \<subseteq> (TYX st' \<union> SX st' \<union> {b}) \<inter> TXY st'" by(auto)
-    also from I owns have "... = {}" by(auto)
-    finally have "(SX st \<inter> TXY st') \<union> (SX st \<inter> \<Delta>BC) = SX st \<inter> \<Delta>BC" by(simp)
-  }
-  txt \<open>@{term "SX st \<inter> \<Delta>BC = {}"} is essential\<close>
-  finally have "SX st \<inter> TXY st = SX st \<inter> \<Delta>BC" .
-  with dBC show "SX st \<inter> TXY st = {}" by(simp)
-
-  from fC have "TYX st \<inter> TXY st = TYX st \<inter> (TXY st' \<union> \<Delta>BC)" by(simp)
-  also have "... = (TYX st \<inter> TXY st') \<union> (TYX st \<inter> \<Delta>BC)" by(auto)
-  also {
-    from ss_A have "TYX st \<inter> TXY st' \<subseteq> (TYX st' \<union> {b}) \<inter> TXY st'" by(auto)
-    also from I owns have "... = {}" by(auto)
-    finally have "(TYX st \<inter> TXY st') \<union> (TYX st \<inter> \<Delta>BC) = TYX st \<inter> \<Delta>BC" by(simp)
-  }
-  txt \<open>@{term "TYX st \<inter> \<Delta>BC = {}"} is essential\<close>
-  finally have "TYX st \<inter> TXY st = TYX st \<inter> \<Delta>BC" .
-  with dAC show "TXY st \<inter> TYX st = {}" by(blast)
-
-  from fB have "TYX st \<inter> (\<Delta>BC \<union> SX st) = TYX st \<inter> (SX st' \<union> \<Delta>AB)" by(simp)
-  also have "... = (TYX st \<inter> SX st') \<union> (TYX st \<inter> \<Delta>AB)" by(auto)
-  also {
-    from ss_A have "TYX st \<inter> SX st' \<subseteq> (TYX st' \<union> {b}) \<inter> SX st'" by(auto)
-    also from I owns have "... = {}" by(auto)
-    finally have "(TYX st \<inter> SX st') \<union> (TYX st \<inter> \<Delta>AB) = TYX st \<inter> \<Delta>AB" by(simp)
-  }
-  txt \<open>@{term "TYX st \<inter> \<Delta>AB = {}"} is essential, given @{term "TYX st \<inter> \<Delta>BC = {}"}.\<close>
-  finally have "TYX st \<inter> (\<Delta>BC \<union> SX st) = TYX st \<inter> \<Delta>AB" .
-  with dAB show "SX st \<inter> TYX st = {}" by auto
-qed
 
 text \<open>
   Both invariants I1 and I2 are preserved by \verb+enqueue+ operations, thus we can 
@@ -426,95 +209,69 @@ text \<open>
 \<close>
 
 lemma CleanQ_Set_enq_x_Invariants :
-  assumes I_holds : "CleanQ_Set_Invariants K rb"  and  X_owned: "b \<in> SX rb"
-    shows "CleanQ_Set_Invariants K (CleanQ_Set_enq_x b rb)"  
-  by (meson I_holds CleanQ_Set_Invariants.simps CleanQ_Set_enq_x_I1 
-            CleanQ_Set_enq_x_I2 X_owned)
-
-lemma CleanQ_Set_enq_x_weak_Invariants :
-  fixes st st' K b
-  assumes I: "CleanQ_Set_Invariants K st'"
-      and rb: "st = CleanQ_Set_enq_x b st'"
-      and frame: "frame_weak (TXY st' \<union> {b},SY st', TYX st', SX st' - {b}) (TXY st, SY st, TYX st, SX st)"
-      and owns: "b \<in> SX st'"
-    shows "CleanQ_Set_Invariants K (CleanQ_Set_enq_x b st)"  
-  by (metis CleanQ_Set_State.ext_inject CleanQ_Set_State.surjective CleanQ_Set_enq_x_Invariants 
-      CleanQ_Set_enq_x_upd Diff_idemp I owns rb sup.right_idem)
-
+assumes I_holds : "CleanQ_Set_Invariants K rb"  and  X_owned: "b \<in> SX rb"
+  shows "CleanQ_Set_Invariants K (CleanQ_Set_enq_x b rb)"  
+  using assms CleanQ_Set_Invariants_def CleanQ_Set_enq_x_I1 CleanQ_Set_enq_x_I2 by metis
 
 lemma CleanQ_Set_enq_y_Invariants :
-  assumes I_holds : "CleanQ_Set_Invariants K rb"  and  X_owned: "b \<in> SY rb"
-    shows "CleanQ_Set_Invariants K (CleanQ_Set_enq_y b rb)"  
-  by (meson I_holds CleanQ_Set_Invariants.simps CleanQ_Set_enq_y_I1 
-            CleanQ_Set_enq_y_I2 X_owned)
-
-lemma CleanQ_Set_enq_y_weak_Invariants :
-  fixes st st' K b
-  assumes I: "CleanQ_Set_Invariants K st'"
-      and rb: "st = CleanQ_Set_enq_y b st'"
-      and frame: "frame_weak (TYX st' \<union> {b},SX st', TXY st', SY st' - {b}) (TYX st, SX st, TXY st, SY st)"
-      and owns: "b \<in> SY st'"
-    shows "CleanQ_Set_Invariants K (CleanQ_Set_enq_y b st)"  
-  by (metis CleanQ_Set_State.ext_inject CleanQ_Set_State.surjective CleanQ_Set_enq_y_Invariants 
-      CleanQ_Set_enq_y_upd Diff_idemp I owns rb sup.right_idem)
+assumes I_holds : "CleanQ_Set_Invariants K rb"  and  X_owned: "b \<in> SY rb"
+  shows "CleanQ_Set_Invariants K (CleanQ_Set_enq_y b rb)"  
+  using assms CleanQ_Set_Invariants_def CleanQ_Set_enq_y_I1 CleanQ_Set_enq_y_I2 by metis
 
 
 text \<open>
-  We can show that the buffers are ending up in the right set under the assumption of the strong
-  frame condition
+  We can show that the buffers are ending up in the right set. Buffer B will end up in 
+  the transfer set, this is trivially true by definition.
 \<close>
 
 lemma CleanQ_Set_enq_x_dst :
-  assumes I_holds : "CleanQ_Set_Invariants K rb"  and  X_owned: "b \<in> SX rb"
-    shows "b \<in> TXY (CleanQ_Set_enq_x b rb)"
+  "b \<in> TXY (CleanQ_Set_enq_x b rb)"
   by (simp add: CleanQ_Set_enq_x_upd)
 
 lemma CleanQ_Set_enq_y_dst :
-  assumes I_holds : "CleanQ_Set_Invariants K rb"  and  Y_owned: "b \<in> SY rb"
-    shows "b \<in> TYX (CleanQ_Set_enq_y b rb)"
+  "b \<in> TYX (CleanQ_Set_enq_y b rb)"
   by (simp add: CleanQ_Set_enq_y_upd)
 
 
 text \<open>
-  Next, we can show that the buffers are not in the other set assuming the strong frame condition
+  Next, we can show that the buffers are not in the other sets
 \<close>
 
 lemma CleanQ_Set_enq_x_ndst1 :
-  assumes I_holds : "CleanQ_Set_Invariants K rb"  and  X_owned: "b \<in> SX rb"
-    shows "b \<notin> SY (CleanQ_Set_enq_x b rb)"
-  by (metis CleanQ_Set_Invariants.elims(2) CleanQ_Set_enq_x_I2 CleanQ_Set_enq_x_dst 
-            I2.elims(2) I_holds Set.set_insert X_owned insert_disjoint(1))
+assumes I_holds : "CleanQ_Set_Invariants K rb"  and  X_owned: "b \<in> SX rb"
+  shows "b \<notin> SY (CleanQ_Set_enq_x b rb)"
+  using I_holds X_owned 
+  unfolding CleanQ_Set_Invariants_simp CleanQ_Set_enq_x_def by(auto)
 
 lemma CleanQ_Set_enq_x_ndst2 :
-  assumes I_holds : "CleanQ_Set_Invariants K rb"  and  X_owned: "b \<in> SX rb"
-    shows "b \<notin> SX (CleanQ_Set_enq_x b rb)"
-  by (metis CleanQ_Set_Invariants.elims(2) CleanQ_Set_enq_x_I2 CleanQ_Set_enq_x_dst 
-            I2.elims(2) I_holds Set.set_insert X_owned insert_disjoint(1))
+assumes I_holds : "CleanQ_Set_Invariants K rb"  and  X_owned: "b \<in> SX rb"
+  shows "b \<notin> SX (CleanQ_Set_enq_x b rb)"
+  using I_holds X_owned 
+  unfolding CleanQ_Set_Invariants_simp CleanQ_Set_enq_x_def by(auto)
 
 lemma CleanQ_Set_enq_x_ndst3 :
-  assumes I_holds : "CleanQ_Set_Invariants K rb"  and  X_owned: "b \<in> SX rb"
-    shows "b \<notin> TYX (CleanQ_Set_enq_x b rb)"
-  by (metis CleanQ_Set_Invariants.elims(2) CleanQ_Set_enq_x_I2 CleanQ_Set_enq_x_dst 
-            I2.elims(2) I_holds Set.set_insert X_owned insert_disjoint(1))
-
+assumes I_holds : "CleanQ_Set_Invariants K rb"  and  X_owned: "b \<in> SX rb"
+  shows "b \<notin> TYX (CleanQ_Set_enq_x b rb)"
+  using I_holds X_owned 
+  unfolding CleanQ_Set_Invariants_simp CleanQ_Set_enq_x_def by(auto)
 
 lemma CleanQ_Set_enq_y_ndst1 :
-  assumes I_holds : "CleanQ_Set_Invariants K rb"  and  Y_owned: "b \<in> SY rb"
-    shows "b \<notin> SX (CleanQ_Set_enq_y b rb)"
-  by (metis CleanQ_Set_Invariants.elims(2) CleanQ_Set_enq_y_I2 CleanQ_Set_enq_y_dst 
-            I2.elims(2) I_holds Set.set_insert Y_owned insert_disjoint(1))
+assumes I_holds : "CleanQ_Set_Invariants K rb"  and  Y_owned: "b \<in> SY rb"
+  shows "b \<notin> SX (CleanQ_Set_enq_y b rb)"
+  using I_holds Y_owned 
+  unfolding CleanQ_Set_Invariants_simp CleanQ_Set_enq_y_def by(auto)
 
 lemma CleanQ_Set_enq_y_ndst2 :
-  assumes I_holds : "CleanQ_Set_Invariants K rb"  and  Y_owned: "b \<in> SY rb"
-    shows "b \<notin> SY (CleanQ_Set_enq_y b rb)"
-  by (metis CleanQ_Set_Invariants.elims(2) CleanQ_Set_enq_y_I2 CleanQ_Set_enq_y_dst 
-            I2.elims(2) I_holds Set.set_insert Y_owned insert_disjoint(1))
+assumes I_holds : "CleanQ_Set_Invariants K rb"  and  Y_owned: "b \<in> SY rb"
+  shows "b \<notin> SY (CleanQ_Set_enq_y b rb)"
+  using I_holds Y_owned 
+  unfolding CleanQ_Set_Invariants_simp CleanQ_Set_enq_y_def by(auto)
 
 lemma CleanQ_Set_enq_y_ndst3 :
-  assumes I_holds : "CleanQ_Set_Invariants K rb"  and  Y_owned: "b \<in> SY rb"
-    shows "b \<notin> TXY (CleanQ_Set_enq_y b rb)"
-  by (metis CleanQ_Set_Invariants.elims(2) CleanQ_Set_enq_y_I2 CleanQ_Set_enq_y_dst 
-            I2.elims(2) I_holds Set.set_insert Y_owned insert_disjoint(1))
+assumes I_holds : "CleanQ_Set_Invariants K rb"  and  Y_owned: "b \<in> SY rb"
+  shows "b \<notin> TXY (CleanQ_Set_enq_y b rb)"
+  using I_holds Y_owned 
+  unfolding CleanQ_Set_Invariants_simp CleanQ_Set_enq_y_def by(auto)
 
 
 text \<open>
@@ -523,20 +280,21 @@ text \<open>
 \<close>
 
 lemma CleanQ_Set_enq_x_result :
-  assumes I_holds : "CleanQ_Set_Invariants K rb"  and  X_owned: "b \<in> SX rb"
-      and CQ: "rb' = CleanQ_Set_enq_x b rb"
-    shows "b \<in> TXY rb' \<and>  b \<notin> SX rb' \<and> b \<notin> SY rb' \<and> b \<notin> TYX rb'"
+assumes I_holds : "CleanQ_Set_Invariants K rb"  and  X_owned: "b \<in> SX rb"
+    and CQ: "rb' = CleanQ_Set_enq_x b rb"
+  shows "b \<in> TXY rb' \<and>  b \<notin> SX rb' \<and> b \<notin> SY rb' \<and> b \<notin> TYX rb'"
   using assms
   by (simp add: CleanQ_Set_enq_x_dst CleanQ_Set_enq_x_ndst1 CleanQ_Set_enq_x_ndst2 
                 CleanQ_Set_enq_x_ndst3)
 
 lemma CleanQ_Set_enq_y_result :
-  assumes I_holds : "CleanQ_Set_Invariants K rb"  and  X_owned: "b \<in> SY rb"
-      and CQ: "rb' = CleanQ_Set_enq_y b rb"
-    shows "b \<in> TYX rb' \<and>  b \<notin> SX rb' \<and> b \<notin> SY rb' \<and> b \<notin> TXY rb'"
+assumes I_holds : "CleanQ_Set_Invariants K rb"  and  X_owned: "b \<in> SY rb"
+    and CQ: "rb' = CleanQ_Set_enq_y b rb"
+  shows "b \<in> TYX rb' \<and>  b \<notin> SX rb' \<and> b \<notin> SY rb' \<and> b \<notin> TXY rb'"
   using assms
   by (simp add: CleanQ_Set_enq_y_dst CleanQ_Set_enq_y_ndst1 CleanQ_Set_enq_y_ndst2 
                 CleanQ_Set_enq_y_ndst3)
+
 
 (* ------------------------------------------------------------------------------------ *)
 subsubsection \<open>Dequeue Operation\<close>
@@ -583,216 +341,25 @@ text \<open>
 \<close>
 
 lemma CleanQ_Set_deq_x_I1 :
-  assumes I1_holds : "I1 rb K"  and  TYX_owned: "b \<in> TYX rb"
-    shows "I1 (CleanQ_Set_deq_x b rb) K"
-  unfolding CleanQ_Set_deq_x_def
-  using I1_holds TYX_owned by auto
+assumes I1_holds : "I1 rb K"  and  TYX_owned: "b \<in> TYX rb"
+  shows "I1 (CleanQ_Set_deq_x b rb) K"
+  using I1_holds TYX_owned unfolding CleanQ_Set_deq_x_def I1_def  by auto
 
 lemma CleanQ_Set_deq_y_I1 :
-  assumes I1_holds : "I1 rb K"  and  TXY_owned: "b \<in> TXY rb"
-    shows "I1 (CleanQ_Set_deq_y b rb) K"
-  unfolding CleanQ_Set_deq_y_def
-  using I1_holds TXY_owned by auto
+assumes I1_holds : "I1 rb K"  and  TXY_owned: "b \<in> TXY rb"
+  shows "I1 (CleanQ_Set_deq_y b rb) K"
+  using I1_holds TXY_owned unfolding CleanQ_Set_deq_y_def I1_def  by auto
 
 lemma CleanQ_Set_deq_x_I2 :
-  assumes  I2_holds : "I2 rb"  and  TYX_owned: "b \<in> TYX rb"
-    shows "I2 (CleanQ_Set_deq_x b rb)"
-  unfolding CleanQ_Set_deq_x_def
-  using I2_holds TYX_owned by auto
+assumes  I2_holds : "I2 rb"  and  TYX_owned: "b \<in> TYX rb"
+  shows "I2 (CleanQ_Set_deq_x b rb)"
+  using I2_holds TYX_owned  unfolding CleanQ_Set_deq_x_def I2_def by auto
 
 lemma CleanQ_Set_deq_y_I2 :
-  assumes  I2_holds : "I2 rb"  and  TXY_owned: "b \<in> TXY rb"
-    shows "I2 (CleanQ_Set_deq_y b rb)"
-  unfolding CleanQ_Set_deq_y_def
-  using I2_holds TXY_owned by auto
+assumes  I2_holds : "I2 rb"  and  TXY_owned: "b \<in> TXY rb"
+  shows "I2 (CleanQ_Set_deq_y b rb)"
+  using I2_holds TXY_owned  unfolding CleanQ_Set_deq_y_def I2_def by auto
 
-text \<open>
-  Similar to enqueue we also have to show the same for dequeue and the weak frame condition
-\<close>
-
-lemma CleanQ_Set_deq_x_weak_I1:
-  fixes st st' K b
-  assumes I: "CleanQ_Set_Invariants K st'"
-      and rb: "st = CleanQ_Set_enq_y b st'"
-      and frame: "frame_weak (TXY st',SY st', TYX st' - {b}, SX st' \<union> {b}) (TXY st, SY st, TYX st, SX st)"
-      and owns: "b \<in> TYX st'"
-    shows "I1 st K"
-proof -
-  from frame obtain \<Delta>AB \<Delta>BC where
-    fA: "TXY st' = \<Delta>AB \<union> TXY st" and
-    fB: "SY st' \<union> \<Delta>AB = \<Delta>BC \<union> SY st" and
-    fC: "(TYX st' - {b}) \<union> \<Delta>BC = TYX st" and
-    fD: "SX st' \<union> {b} = SX st" and
-    dAB: "TXY st \<inter> \<Delta>AB = {}" and
-    dAC: "TXY st \<inter> \<Delta>BC = {}" and
-    dBC: "SY st \<inter> \<Delta>BC = {}"
-    by(auto)
-  from fC have "TYX st = (TYX st' - {b}) \<union> \<Delta>BC" by(simp)
-  hence "SY st  \<union> TYX st = (SY st \<union> \<Delta>BC) \<union> (TYX st' - {b})" by(simp add:ac_simps)
-  with fB have "SY st \<union> TYX st = (SY st' \<union> \<Delta>AB) \<union> (TYX st' - {b})" by(simp add:ac_simps)
-  hence "TXY st \<union> SY st \<union> TYX st = (TXY st \<union> \<Delta>AB) \<union> SY st' \<union> (TYX st' - {b})" by blast
-  with fA have "TXY st \<union> SY st \<union> TYX st = TXY st' \<union> SY st' \<union> (TYX st' - {b})" by(simp add:ac_simps)
-  with fD have "TXY st \<union> SY st \<union> TYX st \<union> SX st = TXY st' \<union> SY st' \<union> (TYX st' - {b}) \<union> (SX st' \<union> {b})" by(simp)
-  with owns have "TXY st \<union> SY st \<union> TYX st \<union> SX st = TXY st' \<union> SY st' \<union> TYX st' \<union> SX st'" by(auto)
-  also from I have "... = K" by auto
-  finally show ?thesis by auto
-qed
-
-lemma CleanQ_Set_deq_y_weak_I1:
-  fixes st st' K b
-  assumes I: "CleanQ_Set_Invariants K st'"
-      and rb: "st = CleanQ_Set_enq_y b st'"
-      and frame: "frame_weak (TYX st',SX st', TXY st' - {b}, SY st' \<union> {b}) (TYX st, SX st, TXY st, SY st)"
-      and owns: "b \<in> TXY st'"
-    shows "I1 st K"
-proof -
-  from frame obtain \<Delta>AB \<Delta>BC where
-    fA: "TYX st' = \<Delta>AB \<union> TYX st" and
-    fB: "SX st' \<union> \<Delta>AB = \<Delta>BC \<union> SX st" and
-    fC: "(TXY st' - {b}) \<union> \<Delta>BC = TXY st" and
-    fD: "SY st' \<union> {b} = SY st" and
-    dAB: "TYX st \<inter> \<Delta>AB = {}" and
-    dAC: "TYX st \<inter> \<Delta>BC = {}" and
-    dBC: "SX st \<inter> \<Delta>BC = {}"
-    by(auto)
-
-  from fC have "TXY st = (TXY st' - {b}) \<union> \<Delta>BC" by(simp)
-  hence "SX st  \<union> TXY st = (SX st \<union> \<Delta>BC) \<union> (TXY st' - {b})" by(simp add:ac_simps)
-  with fB have "SX st \<union> TXY st = (SX st' \<union> \<Delta>AB) \<union> (TXY st' - {b})" by(simp add:ac_simps)
-  hence "TYX st \<union> SX st \<union> TXY st = (TYX st \<union> \<Delta>AB) \<union> SX st' \<union> (TXY st' - {b})" by blast
-  with fA have "TYX st \<union> SX st \<union> TXY st = TYX st' \<union> SX st' \<union> (TXY st' - {b})" by(simp add:ac_simps)
-  with fD have "TYX st \<union> SX st \<union> TXY st \<union> SY st = TYX st' \<union> SX st' \<union> (TXY st' - {b}) \<union> (SY st' \<union> {b})" by(simp)
-  with owns have "TYX st \<union> SX st \<union> TXY st \<union> SY st = TYX st' \<union> SX st' \<union> TXY st' \<union> SY st'" by(auto)
-  also from I have "... = K" by auto
-  finally show ?thesis by auto
-qed
-
-lemma CleanQ_Set_deq_x_weak_I2:
-  fixes st st' K b
-  assumes I: "CleanQ_Set_Invariants K st'"
-      and rb: "st = CleanQ_Set_enq_x b st'"
-      and frame: "frame_weak (TXY st',SY st', TYX st' - {b}, SX st' \<union> {b}) (TXY st, SY st, TYX st, SX st)"
-      and owns: "b \<in> TYX st'"
-    shows "I2 st"
-proof(unfold I2.simps, intro conjI)
-  from frame obtain \<Delta>AB \<Delta>BC where
-    fA: "TXY st' = \<Delta>AB \<union> TXY st" and
-    fB: "SY st' \<union> \<Delta>AB = \<Delta>BC \<union> SY st" and
-    fC: "(TYX st' - {b}) \<union> \<Delta>BC = TYX st" and
-    fD: "SX st' \<union> {b} = SX st" and
-    dAB: "TXY st \<inter> \<Delta>AB = {}" and
-    dAC: "TXY st \<inter> \<Delta>BC = {}" and
-    dBC: "SY st \<inter> \<Delta>BC = {}"
-    by(auto)
-
-  from fA have ss_\<Delta>AB: "\<Delta>AB \<subseteq> TXY st'" by(auto)
-  with fB have ss_\<Delta>BC: "\<Delta>BC \<subseteq> TXY st' \<union> SY st'" by(auto)
-
-  from fA have ss_A: "TXY st \<subseteq> TXY st'" by(auto)
-  from fB ss_\<Delta>AB have ss_B: "SY st \<subseteq> TXY st' \<union> SY st'" by(auto)
-  from fC ss_\<Delta>BC have ss_C: "TYX st \<subseteq> TXY st' \<union> SY st' \<union> (TYX st' - {b})" by(auto)
-
-  from I owns ss_A show "SX st \<inter> TXY st = {}" by(unfold fD[symmetric], auto)
-  from I owns ss_B show "SX st \<inter> SY st = {}" by(unfold fD[symmetric], auto)
-  from I owns ss_C show "SX st \<inter> TYX st = {}" by(unfold fD[symmetric], auto)
-
-  from fC have "SY st \<inter> TYX st = SY st \<inter> ((TYX st' - {b}) \<union> \<Delta>BC)" by(simp)
-  also have "... = (SY st \<inter> (TYX st' - {b})) \<union> (SY st \<inter> \<Delta>BC)" by(auto)
-  also {
-    from ss_B have "SY st \<inter> (TYX st' - {b}) \<subseteq> (TXY st' \<union> SY st') \<inter> TYX st'" by(auto)
-    also from I have "... = {}" by(auto)
-    finally have "(SY st \<inter> (TYX st' - {b})) \<union> (SY st \<inter> \<Delta>BC) = SY st \<inter> \<Delta>BC" by(simp)
-  }
-  txt \<open>@{term "SY st \<inter> \<Delta>BC = {}"} is essential\<close>
-  finally have "SY st \<inter> TYX st = SY st \<inter> \<Delta>BC" .
-  with dBC show "SY st \<inter> TYX st = {}" by simp
-
-  from fC have "TXY st \<inter> TYX st = TXY st \<inter> ((TYX st' - {b}) \<union> \<Delta>BC)" by simp
-  also have "... = (TXY st \<inter> (TYX st' - {b})) \<union> (TXY st \<inter> \<Delta>BC)" by blast
-  also {
-    from ss_A have "TXY st \<inter> (TYX st' - {b}) \<subseteq> (TXY st' \<union> {b}) \<inter> (TYX st' - {b})" by(auto)
-    also from I have "... = {}" by(auto)
-    finally have "(TXY st \<inter> (TYX st' - {b})) \<union> (TXY st \<inter> \<Delta>BC) = TXY st \<inter> \<Delta>BC" by(simp)
-  }
-  txt \<open>@{term "TXY st \<inter> \<Delta>BC = {}"} is essential\<close>
-  finally have "TXY st \<inter> TYX st = TXY st \<inter> \<Delta>BC" .
-  with dAC show "TXY st \<inter> TYX st = {}" by(simp)
-
-  from fB have "TXY st \<inter> (\<Delta>BC \<union> SY st) = TXY st \<inter> (SY st' \<union> \<Delta>AB)" by(simp)
-  also have "... = (TXY st \<inter> SY st') \<union> (TXY st \<inter> \<Delta>AB)" by(auto)
-  also {
-    from ss_A have "TXY st \<inter> SY st' \<subseteq> (TXY st' \<union> {b}) \<inter> SY st'" by(auto)
-    also from I owns have "... = {}" by(auto)
-    finally have "(TXY st \<inter> SY st') \<union> (TXY st \<inter> \<Delta>AB) = TXY st \<inter> \<Delta>AB" by(simp)
-  }
-  txt \<open>@{term "TXY st \<inter> \<Delta>AB = {}"} is essential, given @{term "TXY st \<inter> \<Delta>BC = {}"}.\<close>
-  finally have "TXY st \<inter> (\<Delta>BC \<union> SY st) = TXY st \<inter> \<Delta>AB" .
-  with dAB show " SY st \<inter> TXY st = {}" by(auto)
-qed
-
-
-lemma CleanQ_Set_deq_y_weak_I2:
-  fixes st st' K b
-  assumes I: "CleanQ_Set_Invariants K st'"
-      and rb: "st = CleanQ_Set_enq_y b st'"
-      and frame: "frame_weak (TYX st',SX st', TXY st' - {b}, SY st' \<union> {b}) (TYX st, SX st, TXY st, SY st)"
-      and owns: "b \<in> TXY st'"
-    shows "I2 st"
-proof(unfold I2.simps, intro conjI)
-  from frame obtain \<Delta>AB \<Delta>BC where
-    fA: "TYX st' = \<Delta>AB \<union> TYX st" and
-    fB: "SX st' \<union> \<Delta>AB = \<Delta>BC \<union> SX st" and
-    fC: "(TXY st' - {b}) \<union> \<Delta>BC = TXY st" and
-    fD: "SY st' \<union> {b} = SY st" and
-    dAB: "TYX st \<inter> \<Delta>AB = {}" and
-    dAC: "TYX st \<inter> \<Delta>BC = {}" and
-    dBC: "SX st \<inter> \<Delta>BC = {}"
-    by(auto)
-
-  from fA have ss_\<Delta>AB: "\<Delta>AB \<subseteq> TYX st'" by(auto)
-  with fB have ss_\<Delta>BC: "\<Delta>BC \<subseteq> TYX st' \<union> SX st'" by(auto)
-
-  from fA have ss_A: "TYX st \<subseteq> TYX st'" by(auto)
-  from fB ss_\<Delta>AB have ss_B: "SX st \<subseteq> TYX st' \<union> SX st'" by(auto)
-  from fC ss_\<Delta>BC have ss_C: "TXY st \<subseteq> TYX st' \<union> SX st' \<union> (TXY st' - {b})" by(auto)
-
-  from I owns ss_A show "SY st \<inter> TYX st = {}" by(unfold fD[symmetric], auto)
-  from I owns ss_B show "SX st \<inter> SY st = {}" by(unfold fD[symmetric], auto)
-  from I owns ss_C show "SY st \<inter> TXY st = {}" by(unfold fD[symmetric], auto)
-
-  from fC have "SX st \<inter> TXY st = SX st \<inter> ((TXY st' - {b}) \<union> \<Delta>BC)" by(simp)
-  also have "... = (SX st \<inter> (TXY st' - {b})) \<union> (SX st \<inter> \<Delta>BC)" by(auto)
-  also {
-    from ss_B have "SX st \<inter> (TXY st' - {b}) \<subseteq> (TYX st' \<union> SX st') \<inter> TXY st'" by(auto)
-    also from I have "... = {}" by(auto)
-    finally have "(SX st \<inter> (TXY st' - {b})) \<union> (SX st \<inter> \<Delta>BC) = SX st \<inter> \<Delta>BC" by(simp)
-  }
-  txt \<open>@{term "SX st \<inter> \<Delta>BC = {}"} is essential\<close>
-  finally have "SX st \<inter> TXY st = SX st \<inter> \<Delta>BC" .
-  with dBC show "SX st \<inter> TXY st = {}" by simp
-
-  from fC have "TYX st \<inter> TXY st = TYX st \<inter> ((TXY st' - {b}) \<union> \<Delta>BC)" by simp
-  also have "... = (TYX st \<inter> (TXY st' - {b})) \<union> (TYX st \<inter> \<Delta>BC)" by blast
-  also {
-    from ss_A have "TYX st \<inter> (TXY st' - {b}) \<subseteq> (TYX st' \<union> {b}) \<inter> (TXY st' - {b})" by(auto)
-    also from I have "... = {}" by(auto)
-    finally have "(TYX st \<inter> (TXY st' - {b})) \<union> (TYX st \<inter> \<Delta>BC) = TYX st \<inter> \<Delta>BC" by(simp)
-  }
-  txt \<open>@{term "TYX st \<inter> \<Delta>BC = {}"} is essential\<close>
-  finally have "TYX st \<inter> TXY st = TYX st \<inter> \<Delta>BC" .
-  with dAC show "TXY st \<inter> TYX st = {}" by auto
-
-  from fB have "TYX st \<inter> (\<Delta>BC \<union> SX st) = TYX st \<inter> (SX st' \<union> \<Delta>AB)" by(simp)
-  also have "... = (TYX st \<inter> SX st') \<union> (TYX st \<inter> \<Delta>AB)" by(auto)
-  also {
-    from ss_A have "TYX st \<inter> SX st' \<subseteq> (TYX st' \<union> {b}) \<inter> SX st'" by(auto)
-    also from I owns have "... = {}" by(auto)
-    finally have "(TYX st \<inter> SX st') \<union> (TYX st \<inter> \<Delta>AB) = TYX st \<inter> \<Delta>AB" by(simp)
-  }
-  txt \<open>@{term "TYX st \<inter> \<Delta>AB = {}"} is essential, given @{term "TYX st \<inter> \<Delta>BC = {}"}.\<close>
-  finally have "TYX st \<inter> (\<Delta>BC \<union> SX st) = TYX st \<inter> \<Delta>AB" .
-  with dAB show " SX st \<inter> TYX st = {}" by(auto)
-qed
 
 text \<open>
   Both invariants I1 and I2 are preserved by dequeue operations, thus we can combine them 
@@ -800,52 +367,29 @@ text \<open>
 \<close>
 
 lemma CleanQ_Set_deq_x_Invariants :
-  assumes I_holds : "CleanQ_Set_Invariants K rb"  and  TYX_owned: "b \<in> TYX rb"
-    shows "CleanQ_Set_Invariants K (CleanQ_Set_deq_x b rb)" 
-  by (meson CleanQ_Set_Invariants.simps CleanQ_Set_deq_x_I1 CleanQ_Set_deq_x_I2 I_holds 
-            TYX_owned)
-
-lemma CleanQ_Set_deq_x_weak_Invariants :
-  fixes st st' K b
-  assumes I: "CleanQ_Set_Invariants K st'"
-      and rb: "st = CleanQ_Set_deq_x b st'"
-      and frame: "frame_weak (TXY st' ,SY st', TYX st' - {b}, SX st' \<union> {b}) (TXY st, SY st, TYX st, SX st)"
-      and owns: "b \<in> TYX st'"
-    shows "CleanQ_Set_Invariants K (CleanQ_Set_deq_x b st)"  
-  by (metis CleanQ_Set_State.select_convs(2) CleanQ_Set_State.select_convs(3) 
-      CleanQ_Set_State.select_convs(4) CleanQ_Set_deq_x_Invariants CleanQ_Set_deq_x_upd Diff_idemp I 
-      frame frame_weak.simps owns rb sup.right_idem)
+assumes I_holds : "CleanQ_Set_Invariants K rb"  and  TYX_owned: "b \<in> TYX rb"
+  shows "CleanQ_Set_Invariants K (CleanQ_Set_deq_x b rb)" 
+  using assms unfolding CleanQ_Set_Invariants_def I1_def I2_def CleanQ_Set_deq_x_def by auto
+   
 
 lemma CleanQ_Set_deq_y_Invariants :
-  assumes I_holds : "CleanQ_Set_Invariants K rb"  and  TXY_owned: "b \<in> TXY rb"
-    shows "CleanQ_Set_Invariants K (CleanQ_Set_deq_y b rb)" 
-  by (meson CleanQ_Set_Invariants.simps CleanQ_Set_deq_y_I1 CleanQ_Set_deq_y_I2 I_holds
-            TXY_owned)
+assumes I_holds : "CleanQ_Set_Invariants K rb"  and  TXY_owned: "b \<in> TXY rb"
+  shows "CleanQ_Set_Invariants K (CleanQ_Set_deq_y b rb)" 
+  using assms unfolding CleanQ_Set_Invariants_def I1_def I2_def CleanQ_Set_deq_y_def by auto
 
-lemma CleanQ_Set_deq_y_weak_Invariants :
-  fixes st st' K b
-  assumes I: "CleanQ_Set_Invariants K st'"
-      and rb: "st = CleanQ_Set_deq_y b st'"
-      and frame: "frame_weak (TYX st' ,SX st', TXY st' - {b}, SY st' \<union> {b}) (TYX st, SX st, TXY st, SY st)"
-      and owns: "b \<in> TXY st'"
-    shows "CleanQ_Set_Invariants K (CleanQ_Set_deq_y b st)"   
-  by (metis CleanQ_Set_State.select_convs(1) CleanQ_Set_State.select_convs(3) 
-      CleanQ_Set_State.select_convs(4) CleanQ_Set_deq_y_Invariants CleanQ_Set_deq_y_upd Diff_idemp I 
-      frame frame_weak.simps owns rb sup.right_idem)
 
 text \<open>
-  We can show that the buffers are ending up in the right set
+  We can show that the buffers are ending up in the right set. The dequeued buffer goes
+  into the SX or SY sets respectively. This is by definition, and thus trivial.
 \<close>
 
 lemma CleanQ_Set_deq_x_dst :
-  assumes I_holds : "CleanQ_Set_Invariants K rb"  and  X_owned: "b \<in> TYX rb"
-    shows "b \<in> SX (CleanQ_Set_deq_x b rb)"
+  "b \<in> SX (CleanQ_Set_deq_x b rb)"
   by (simp add: CleanQ_Set_deq_x_upd)
 
 
 lemma CleanQ_Set_deq_y_dst :
-  assumes I_holds : "CleanQ_Set_Invariants K rb"  and  Y_owned: "b \<in> TXY rb"
-    shows "b \<in> SY (CleanQ_Set_deq_y b rb)"
+  "b \<in> SY (CleanQ_Set_deq_y b rb)"
   by (simp add: CleanQ_Set_deq_y_upd)
 
 
@@ -854,40 +398,34 @@ text \<open>
 \<close>
 
 lemma CleanQ_Set_deq_x_ndst1 :
-  assumes I_holds : "CleanQ_Set_Invariants K rb"  and  X_owned: "b \<in> TYX rb"
-    shows "b \<notin> SY (CleanQ_Set_deq_x b rb)"
-  by (metis CleanQ_Set_Invariants.elims(2) CleanQ_Set_deq_x_I2 CleanQ_Set_deq_x_dst 
-            I2.elims(2) I_holds X_owned disjoint_insert(1) mk_disjoint_insert)
+assumes I_holds : "CleanQ_Set_Invariants K rb"  and  X_owned: "b \<in> TYX rb"
+  shows "b \<notin> SY (CleanQ_Set_deq_x b rb)"
+  using assms unfolding CleanQ_Set_deq_x_def CleanQ_Set_Invariants_simp by(auto)
 
 lemma CleanQ_Set_deq_x_ndst2 :
-  assumes I_holds : "CleanQ_Set_Invariants K rb"  and  X_owned: "b \<in> TYX rb"
-    shows "b \<notin> TXY (CleanQ_Set_deq_x b rb)"
-  by (metis CleanQ_Set_Invariants.elims(2) CleanQ_Set_deq_x_I2 CleanQ_Set_deq_x_dst 
-            I2.elims(2) I_holds X_owned disjoint_insert(1) mk_disjoint_insert)
+assumes I_holds : "CleanQ_Set_Invariants K rb"  and  X_owned: "b \<in> TYX rb"
+  shows "b \<notin> TXY (CleanQ_Set_deq_x b rb)"
+  using assms unfolding CleanQ_Set_deq_x_def CleanQ_Set_Invariants_simp by(auto)
 
 lemma CleanQ_Set_deq_x_ndst3 :
-  assumes I_holds : "CleanQ_Set_Invariants K rb"  and  X_owned: "b \<in> TYX rb"
-    shows "b \<notin> TYX (CleanQ_Set_deq_x b rb)"
-  by (metis CleanQ_Set_Invariants.elims(2) CleanQ_Set_deq_x_I2 CleanQ_Set_deq_x_dst 
-            I2.elims(2) I_holds X_owned disjoint_insert(1) mk_disjoint_insert)
+assumes I_holds : "CleanQ_Set_Invariants K rb"  and  X_owned: "b \<in> TYX rb"
+  shows "b \<notin> TYX (CleanQ_Set_deq_x b rb)"
+  using assms unfolding CleanQ_Set_deq_x_def CleanQ_Set_Invariants_simp by(auto)
 
 lemma CleanQ_Set_deq_y_ndst1 :
-  assumes I_holds : "CleanQ_Set_Invariants K rb"  and  Y_owned: "b \<in> TXY rb"
-    shows "b \<notin> SX (CleanQ_Set_deq_y b rb)"
-  by (metis CleanQ_Set_Invariants.elims(2) CleanQ_Set_deq_y_I2 CleanQ_Set_deq_y_dst 
-      I2.elims(2) I_holds Set.set_insert Y_owned insert_disjoint(1))
+assumes I_holds : "CleanQ_Set_Invariants K rb"  and  Y_owned: "b \<in> TXY rb"
+  shows "b \<notin> SX (CleanQ_Set_deq_y b rb)"
+  using assms unfolding CleanQ_Set_deq_y_def CleanQ_Set_Invariants_simp by(auto)
 
 lemma CleanQ_Set_deq_y_ndst2 :
-  assumes I_holds : "CleanQ_Set_Invariants K rb"  and  Y_owned: "b \<in> TXY rb"
-    shows "b \<notin> TYX (CleanQ_Set_deq_y b rb)"
-  by (metis CleanQ_Set_Invariants.elims(2) CleanQ_Set_deq_y_I2 CleanQ_Set_deq_y_dst 
-      I2.elims(2) I_holds Set.set_insert Y_owned insert_disjoint(1))
+assumes I_holds : "CleanQ_Set_Invariants K rb"  and  Y_owned: "b \<in> TXY rb"
+  shows "b \<notin> TYX (CleanQ_Set_deq_y b rb)"
+  using assms unfolding CleanQ_Set_deq_y_def CleanQ_Set_Invariants_simp by(auto)
 
 lemma CleanQ_Set_deq_y_ndst3 :
-  assumes I_holds : "CleanQ_Set_Invariants K rb"  and  Y_owned: "b \<in> TXY rb"
-    shows "b \<notin> TXY (CleanQ_Set_deq_y b rb)"
-  by (metis CleanQ_Set_Invariants.elims(2) CleanQ_Set_deq_y_I2 CleanQ_Set_deq_y_dst 
-      I2.elims(2) I_holds Set.set_insert Y_owned insert_disjoint(1))
+assumes I_holds : "CleanQ_Set_Invariants K rb"  and  Y_owned: "b \<in> TXY rb"
+  shows "b \<notin> TXY (CleanQ_Set_deq_y b rb)"
+  using assms unfolding CleanQ_Set_deq_y_def CleanQ_Set_Invariants_simp by(auto)
 
 
 text \<open>
@@ -896,21 +434,32 @@ text \<open>
 \<close>
 
 lemma CleanQ_Set_deq_x_result :
-  assumes I_holds : "CleanQ_Set_Invariants K rb"  and  YX_owned: "b \<in> TYX rb"
-      and CQ: "rb' = CleanQ_Set_deq_x b rb"
-    shows "b \<in> SX rb' \<and>  b \<notin> SY rb' \<and> b \<notin> TXY rb' \<and> b \<notin> TYX rb'"
+assumes I_holds : "CleanQ_Set_Invariants K rb"  and  YX_owned: "b \<in> TYX rb"
+    and CQ: "rb' = CleanQ_Set_deq_x b rb"
+  shows "b \<in> SX rb' \<and>  b \<notin> SY rb' \<and> b \<notin> TXY rb' \<and> b \<notin> TYX rb'"
   using assms
   by (simp add: CleanQ_Set_deq_x_dst CleanQ_Set_deq_x_ndst1 CleanQ_Set_deq_x_ndst2 
                 CleanQ_Set_deq_x_ndst3)
 
 lemma CleanQ_Set_deq_y_result :
-  assumes I_holds : "CleanQ_Set_Invariants K rb"  and  YX_owned: "b \<in> TXY rb"
-      and CQ: "rb' = CleanQ_Set_deq_y b rb"
-    shows "b \<in> SY rb' \<and>  b \<notin> SX rb' \<and> b \<notin> TXY rb' \<and> b \<notin> TYX rb'"
+assumes I_holds : "CleanQ_Set_Invariants K rb"  and  YX_owned: "b \<in> TXY rb"
+    and CQ: "rb' = CleanQ_Set_deq_y b rb"
+  shows "b \<in> SY rb' \<and>  b \<notin> SX rb' \<and> b \<notin> TXY rb' \<and> b \<notin> TYX rb'"
   using assms
   by (simp add: CleanQ_Set_deq_y_dst CleanQ_Set_deq_y_ndst1 CleanQ_Set_deq_y_ndst2 
                 CleanQ_Set_deq_y_ndst3)
 
+
+(* ------------------------------------------------------------------------------------ *)
+subsubsection \<open>Lemmas Summaries\<close>
+(* ------------------------------------------------------------------------------------ *)
+
+text \<open>
+  We define a few lemmas and lemma groups which simplify the proofs
+\<close>
+
+lemmas CleanQ_Set_ops = CleanQ_Set_deq_x_def CleanQ_Set_deq_y_def 
+                        CleanQ_Set_enq_x_def CleanQ_Set_enq_y_def
 
 
 (* ==================================================================================== *)
@@ -918,9 +467,11 @@ subsection \<open>Multistep State Transition Operations\<close>
 (* ==================================================================================== *)
 
 text \<open>
-  We now define the semantics of enqueuing and dequing multiple buffers. 
+  We now define the semantics of enqueuing and dequing multiple buffers. This is useful
+  when talking about concurrency: The other side may enqueue and/or dequeue multiple
+  buffers at once, as observed by the one side. We therefore define the \verb+enqueue+
+  and \verb+dequeue+ operation to operation on a set of buffers.
 \<close>
-
 
 
 (* ------------------------------------------------------------------------------------ *)
@@ -936,7 +487,7 @@ definition CleanQ_Set_enq_n_y :: "'a set \<Rightarrow> 'a CleanQ_Set_State \<Rig
 
 
 text \<open>
-  We can inductively describe the effects on the enqueue N operation:
+  We can inductively describe the effects on the enqueue N operation, by taking the 
 \<close>
 
 lemma CleanQ_Set_enq_n_x_ind:
@@ -961,65 +512,75 @@ lemma CleanQ_Set_enq_n_y_ind_list:
 
 
 text \<open>
+  The inductive definition can be commuted:
+\<close>
+
+lemma CleanQ_Set_enq_n_x_commute:
+  "CleanQ_Set_enq_x b (CleanQ_Set_enq_n_x B rb) = CleanQ_Set_enq_n_x B (CleanQ_Set_enq_x b rb)"
+  unfolding CleanQ_Set_enq_n_x_def CleanQ_Set_enq_x_def
+  by (simp, metis Diff_insert Diff_insert2)
+
+lemma CleanQ_Set_enq_n_y_commute:
+  "CleanQ_Set_enq_y b (CleanQ_Set_enq_n_y B rb) = CleanQ_Set_enq_n_y B (CleanQ_Set_enq_y b rb)"
+  unfolding CleanQ_Set_enq_n_y_def CleanQ_Set_enq_y_def
+  by (simp, metis Diff_insert Diff_insert2)
+
+
+text \<open>
   Like the single step enqueue operation, we can show that doing this multi-step, still
-  preserves all the invariants.
+  preserves invariant I1 and I2..
 \<close>
 
 lemma CleanQ_Set_enq_n_x_I1 :
-  assumes I1_holds: "I1 rb K"  and  X_owned: "\<forall>b \<in> B. b \<in> SX rb" 
-    shows "I1 (CleanQ_Set_enq_n_x B rb) K"
-  unfolding CleanQ_Set_enq_n_x_def 
-  using I1_holds X_owned by auto
+assumes I1_holds: "I1 rb K"  and  X_owned: "\<forall>b \<in> B. b \<in> SX rb" 
+  shows "I1 (CleanQ_Set_enq_n_x B rb) K"
+  using I1_holds X_owned unfolding CleanQ_Set_enq_n_x_def I1_def by auto
 
 lemma CleanQ_Set_enq_n_y_I1 :
-  assumes I1_holds: "I1 rb K"  and  Y_owned: "\<forall>b \<in> B. b \<in> SY rb" 
-    shows "I1 (CleanQ_Set_enq_n_y B rb) K"
-  unfolding CleanQ_Set_enq_n_y_def 
-  using I1_holds Y_owned by auto
+assumes I1_holds: "I1 rb K"  and  Y_owned: "\<forall>b \<in> B. b \<in> SY rb" 
+  shows "I1 (CleanQ_Set_enq_n_y B rb) K"
+  using I1_holds Y_owned unfolding CleanQ_Set_enq_n_y_def I1_def by auto
 
 lemma CleanQ_Set_enq_n_x_I2 :
-  assumes I2_holds: "I2 rb"  and  X_owned: "\<forall>b \<in> B. b \<in> SX rb" 
+assumes I2_holds: "I2 rb"  and  X_owned: "\<forall>b \<in> B. b \<in> SX rb" 
   shows "I2 (CleanQ_Set_enq_n_x B rb)"
-  unfolding CleanQ_Set_enq_n_x_def
-  using I2_holds X_owned by(auto)
+  using I2_holds X_owned unfolding CleanQ_Set_enq_n_x_def I2_def by auto
 
 lemma CleanQ_Set_enq_n_y_I2 :
-  assumes I2_holds: "I2 rb"  and  Y_owned: "\<forall>b \<in> B. b \<in> SY rb" 
+assumes I2_holds: "I2 rb"  and  Y_owned: "\<forall>b \<in> B. b \<in> SY rb" 
   shows "I2 (CleanQ_Set_enq_n_y B rb)"
-  unfolding CleanQ_Set_enq_n_y_def
-  using I2_holds Y_owned by(auto)
+  using I2_holds Y_owned unfolding CleanQ_Set_enq_n_y_def I2_def by auto
+
 
 text \<open>
-  Likewise, we can show that the \verb+CleanQ_Set_Invariants" are preserved
+  Likewise, we can show that the \verb+CleanQ_Set_Invariants" are preserved by combining
+  the lemmas above:
 \<close>
 
 lemma CleanQ_Set_enq_n_x_Invariants :
 assumes I_holds : "CleanQ_Set_Invariants K rb"  and  X_owned: "\<forall>b \<in> B. b \<in> SX rb" 
   shows "CleanQ_Set_Invariants K (CleanQ_Set_enq_n_x B rb)"  
-  using I_holds X_owned CleanQ_Set_enq_n_x_I1 CleanQ_Set_enq_n_x_I2
-        CleanQ_Set_Invariants.simps 
+  using assms CleanQ_Set_enq_n_x_I1 CleanQ_Set_enq_n_x_I2 CleanQ_Set_Invariants_simp
   by blast
 
 lemma CleanQ_Set_enq_n_y_Invariants :
 assumes I_holds : "CleanQ_Set_Invariants K rb"  and  Y_owned: "\<forall>b \<in> B. b \<in> SY rb" 
   shows "CleanQ_Set_Invariants K (CleanQ_Set_enq_n_y B rb)"  
-  using I_holds Y_owned CleanQ_Set_enq_n_y_I1 CleanQ_Set_enq_n_y_I2
-        CleanQ_Set_Invariants.simps 
+  using assms CleanQ_Set_enq_n_y_I1 CleanQ_Set_enq_n_y_I2 CleanQ_Set_Invariants_simp 
   by blast
 
 
 text \<open>
-  We can now show that all buffers in the set $B$ are ending up in the transfer sets.
+  We can now show that all buffers in the set $B$ are ending up in the transfer sets. 
+  Not this is trivially true, as enqueue inserts those buffers into the transfer set. 
 \<close>
 
 lemma CleanQ_Set_enq_n_x_dst :
-assumes I_holds : "CleanQ_Set_Invariants K rb"  and  X_owned: "\<forall>b \<in> B. b \<in> SX rb" 
-  shows "\<forall> b \<in> B. b \<in> TXY (CleanQ_Set_enq_n_x B rb)"
+  "\<forall>b \<in> B. b \<in> TXY (CleanQ_Set_enq_n_x B rb)"
   by (simp add: CleanQ_Set_enq_n_x_def)
 
 lemma CleanQ_Set_enq_n_y_dst :
-assumes I_holds : "CleanQ_Set_Invariants K rb"  and  Y_owned: "\<forall>b \<in> B. b \<in> SY rb" 
-  shows "\<forall> b \<in> B. b \<in> TYX (CleanQ_Set_enq_n_y B rb)"
+  "\<forall> b \<in> B. b \<in> TYX (CleanQ_Set_enq_n_y B rb)"
   by (simp add: CleanQ_Set_enq_n_y_def)
 
 text \<open>
@@ -1029,52 +590,52 @@ text \<open>
 lemma CleanQ_Set_enq_n_x_ndst1 :
   assumes I_holds : "CleanQ_Set_Invariants K rb"  and  X_owned: "\<forall>b \<in> B. b \<in> SX rb" 
   shows "\<forall>b \<in> B. b \<notin> SY (CleanQ_Set_enq_n_x B rb)"
-  unfolding CleanQ_Set_enq_n_x_def using I_holds X_owned I2.elims(2) by auto
+  using assms unfolding CleanQ_Set_Invariants_simp CleanQ_Set_enq_n_x_def by(auto)
 
 lemma CleanQ_Set_enq_n_x_ndst2 :
   assumes I_holds : "CleanQ_Set_Invariants K rb"  and  X_owned: "\<forall>b \<in> B. b \<in> SX rb" 
   shows "\<forall>b \<in> B. b \<notin> SX (CleanQ_Set_enq_n_x B rb)"
-  unfolding CleanQ_Set_enq_n_x_def using I_holds X_owned I2.elims(2) by auto
+  using assms unfolding CleanQ_Set_Invariants_simp CleanQ_Set_enq_n_x_def by(auto)
 
 lemma CleanQ_Set_enq_n_x_ndst3 :
   assumes I_holds : "CleanQ_Set_Invariants K rb"  and  X_owned: "\<forall>b \<in> B. b \<in> SX rb" 
   shows "\<forall>b \<in> B. b \<notin> TYX (CleanQ_Set_enq_n_x B rb)"
-  unfolding CleanQ_Set_enq_n_x_def using I_holds X_owned I2.elims(2) by auto
+  using assms unfolding CleanQ_Set_Invariants_simp CleanQ_Set_enq_n_x_def by(auto)
 
 lemma CleanQ_Set_enq_n_y_ndst1 :
   assumes I_holds : "CleanQ_Set_Invariants K rb"  and  Y_owned: "\<forall>b \<in> B. b \<in> SY rb" 
   shows "\<forall>b \<in> B. b \<notin> SY (CleanQ_Set_enq_n_y B rb)"
-  unfolding CleanQ_Set_enq_n_y_def using I_holds Y_owned I2.elims(2) by auto
+  using assms unfolding CleanQ_Set_Invariants_simp CleanQ_Set_enq_n_y_def by(auto)
 
 lemma CleanQ_Set_enq_n_y_ndst2 :
   assumes I_holds : "CleanQ_Set_Invariants K rb"  and  Y_owned: "\<forall>b \<in> B. b \<in> SY rb" 
   shows "\<forall>b \<in> B. b \<notin> SX (CleanQ_Set_enq_n_y B rb)"
-  unfolding CleanQ_Set_enq_n_y_def using I_holds Y_owned I2.elims(2) by auto
+  using assms unfolding CleanQ_Set_Invariants_simp CleanQ_Set_enq_n_y_def by(auto)
 
 lemma CleanQ_Set_enq_n_y_ndst3 :
   assumes I_holds : "CleanQ_Set_Invariants K rb"  and  Y_owned: "\<forall>b \<in> B. b \<in> SY rb" 
   shows "\<forall>b \<in> B. b \<notin> TXY (CleanQ_Set_enq_n_y B rb)"
-  unfolding CleanQ_Set_enq_n_y_def using I_holds Y_owned I2.elims(2) by auto
+  using assms unfolding CleanQ_Set_Invariants_simp CleanQ_Set_enq_n_y_def by(auto)
 
 
 text \<open>
-  We can now combine the lemmas above to obtain the result of the multi-step enqueue
-  operation.
+  We can now combine the lemmas above to obtain the result of the multi-step 
+  \verb+ enqueue+  operation.
 \<close>
 
 lemma CleanQ_Set_enq_n_x_result :
-  assumes I_holds : "CleanQ_Set_Invariants K rb"  and  X_owned: "\<forall>b \<in> B. b \<in> SX rb" 
-      and CQ: "rb' = CleanQ_Set_enq_n_x B rb"
-    shows "\<forall>b \<in> B. b \<in> TXY rb' \<and>  b \<notin> SX rb' \<and> b \<notin> SY rb' \<and> b \<notin> TYX rb'"
+assumes I_holds : "CleanQ_Set_Invariants K rb"  and  X_owned: "\<forall>b \<in> B. b \<in> SX rb" 
+    and CQ: "rb' = CleanQ_Set_enq_n_x B rb"
+  shows "\<forall>b \<in> B. b \<in> TXY rb' \<and>  b \<notin> SX rb' \<and> b \<notin> SY rb' \<and> b \<notin> TYX rb'"
   using assms
   by (simp add: CleanQ_Set_enq_n_x_dst CleanQ_Set_enq_n_x_ndst1 CleanQ_Set_enq_n_x_ndst2 
                 CleanQ_Set_enq_n_x_ndst3)
 
 
 lemma CleanQ_Set_enq_n_y_result :
-  assumes I_holds : "CleanQ_Set_Invariants K rb"  and  Y_owned: "\<forall>b \<in> B. b \<in> SY rb" 
-      and CQ: "rb' = CleanQ_Set_enq_n_y B rb"
-    shows "\<forall>b \<in> B. b \<in> TYX rb' \<and>  b \<notin> SX rb' \<and> b \<notin> SY rb' \<and> b \<notin> TXY rb'"
+assumes I_holds : "CleanQ_Set_Invariants K rb"  and  Y_owned: "\<forall>b \<in> B. b \<in> SY rb" 
+    and CQ: "rb' = CleanQ_Set_enq_n_y B rb"
+  shows "\<forall>b \<in> B. b \<in> TYX rb' \<and>  b \<notin> SX rb' \<and> b \<notin> SY rb' \<and> b \<notin> TXY rb'"
   using assms
   by (simp add: CleanQ_Set_enq_n_y_dst CleanQ_Set_enq_n_y_ndst1 CleanQ_Set_enq_n_y_ndst2 
                 CleanQ_Set_enq_n_y_ndst3)
@@ -1086,8 +647,8 @@ subsubsection \<open>Dequeue-N Operation\<close>
 
 
 text \<open>
-  We now define the the effects of dequenuing  multiple buffers at once from the 
-  transfer set. 
+  We now define the the effects of performing a \verb+dequeue+ of  multiple buffers at 
+  once from the transfer set. 
 \<close>
 
 definition CleanQ_Set_deq_n_x :: "'a set \<Rightarrow> 'a CleanQ_Set_State \<Rightarrow> 'a CleanQ_Set_State"
@@ -1098,6 +659,10 @@ definition CleanQ_Set_deq_n_y :: "'a set \<Rightarrow> 'a CleanQ_Set_State \<Rig
   where "CleanQ_Set_deq_n_y B rb = \<lparr> SX = (SX rb), SY = (SY rb) \<union> B, 
                                    TXY = (TXY rb) - B, TYX = (TYX rb) \<rparr>"
 
+
+text \<open>
+  We can define this in an inductive way:
+\<close>
 
 lemma CleanQ_Set_deq_n_x_ind:
   "CleanQ_Set_deq_n_x ({b} \<union> B) rb = CleanQ_Set_deq_x b (CleanQ_Set_deq_n_x B rb)"
@@ -1117,60 +682,60 @@ lemma CleanQ_Set_deq_n_y_ind_list:
 
 
 text \<open>
-  We can now show that the multi-dequeue operation preserves the invariants 
+  The multi-step \verb+dequeue_n+ operation perserves the invariant I1 and I2.
 \<close>
 
 lemma CleanQ_Set_deq_n_x_I1 :
 assumes I1_holds : "I1 rb K"  and  TYX_owned: "\<forall>b \<in> B. b \<in> TYX rb"
   shows "I1 (CleanQ_Set_deq_n_x B rb) K"
-  unfolding CleanQ_Set_deq_n_x_def using I1_holds TYX_owned by auto
+  using assms unfolding CleanQ_Set_deq_n_x_def I1_def by(auto)
 
 lemma CleanQ_Set_deq_n_y_I1 :
 assumes I1_holds : "I1 rb K"  and  TXY_owned: "\<forall>b \<in> B. b \<in> TXY rb"
   shows "I1 (CleanQ_Set_deq_n_y B rb) K"
-  unfolding CleanQ_Set_deq_n_y_def using I1_holds TXY_owned by auto
+  using assms unfolding CleanQ_Set_deq_n_y_def I1_def by(auto)
 
 lemma CleanQ_Set_deq_n_x_I2 :
-assumes  I2_holds : "I2 rb"  and  TYX_owned: "\<forall>b \<in> B. b \<in> TYX rb"
+assumes I2_holds : "I2 rb"  and  TYX_owned: "\<forall>b \<in> B. b \<in> TYX rb"
   shows "I2 (CleanQ_Set_deq_n_x B rb)"
-  unfolding CleanQ_Set_deq_n_x_def
-  using I2_holds TYX_owned disjoint_iff_not_equal by fastforce
+  using assms unfolding CleanQ_Set_deq_n_x_def I2_def by(auto)
 
 lemma CleanQ_Set_deq_n_y_I2 :
-assumes  I2_holds : "I2 rb"  and  TYX_owned: "\<forall>b \<in> B. b \<in> TXY rb"
+assumes I2_holds : "I2 rb"  and  TYX_owned: "\<forall>b \<in> B. b \<in> TXY rb"
   shows "I2 (CleanQ_Set_deq_n_y B rb)"
-  unfolding CleanQ_Set_deq_n_y_def
-  using I2_holds TYX_owned disjoint_iff_not_equal by fastforce
+  using assms unfolding CleanQ_Set_deq_n_y_def I2_def by(auto)
+
 
 text \<open>
   And we can combine the lemmas above to get show that the set invariant is preserved
+  by the \verb+dequeue_n+ operation:
 \<close>
 
 lemma CleanQ_Set_deq_n_x_Invariants :
-  assumes I_holds : "CleanQ_Set_Invariants K rb"  and  TYX_owned: "\<forall>b \<in> B. b \<in> TYX rb"
-    shows "CleanQ_Set_Invariants K (CleanQ_Set_deq_n_x B rb)" 
-  by (meson CleanQ_Set_Invariants.simps CleanQ_Set_deq_n_x_I1 CleanQ_Set_deq_n_x_I2 I_holds 
-            TYX_owned)
+assumes I_holds : "CleanQ_Set_Invariants K rb"  and  TYX_owned: "\<forall>b \<in> B. b \<in> TYX rb"
+  shows "CleanQ_Set_Invariants K (CleanQ_Set_deq_n_x B rb)" 
+  using assms CleanQ_Set_deq_n_x_I1 CleanQ_Set_deq_n_x_I2 I_holds 
+  unfolding CleanQ_Set_Invariants_def by(auto)
+
 
 lemma CleanQ_Set_deq_n_y_Invariants :
-  assumes I_holds : "CleanQ_Set_Invariants K rb"  and  TXY_owned: "\<forall>b \<in> B. b \<in> TXY rb"
-    shows "CleanQ_Set_Invariants K (CleanQ_Set_deq_n_y B rb)" 
-  by (meson CleanQ_Set_Invariants.simps CleanQ_Set_deq_n_y_I1 CleanQ_Set_deq_n_y_I2 I_holds 
-            TXY_owned)
+assumes I_holds : "CleanQ_Set_Invariants K rb"  and  TXY_owned: "\<forall>b \<in> B. b \<in> TXY rb"
+  shows "CleanQ_Set_Invariants K (CleanQ_Set_deq_n_y B rb)" 
+  using assms CleanQ_Set_deq_n_y_I1 CleanQ_Set_deq_n_y_I2 I_holds 
+  unfolding CleanQ_Set_Invariants_def by(auto)
 
 
 text \<open>
-  We can now talk about where the buffers end up when doing a multi-dequeue operation
+  We can now talk about where the buffers end up when performing \verb+dequeue_n+ 
+  This is by definition trivial.
 \<close>
 
 lemma CleanQ_Set_deq_n_x_dst :
-  assumes I_holds : "CleanQ_Set_Invariants K rb"  and  X_owned: "\<forall>b \<in> B. b \<in> TYX rb"
-    shows "\<forall> b \<in> B. b \<in> SX (CleanQ_Set_deq_n_x B rb)"
+  "\<forall> b \<in> B. b \<in> SX (CleanQ_Set_deq_n_x B rb)"
   unfolding CleanQ_Set_deq_n_x_def by(auto)
 
 lemma CleanQ_Set_deq_n_y_dst :
-  assumes I_holds : "CleanQ_Set_Invariants K rb"  and  X_owned: "\<forall>b \<in> B. b \<in> TXY rb"
-    shows "\<forall> b \<in> B. b \<in> SY (CleanQ_Set_deq_n_y B rb)"
+  "\<forall> b \<in> B. b \<in> SY (CleanQ_Set_deq_n_y B rb)"
   unfolding CleanQ_Set_deq_n_y_def by(auto)
 
 text \<open>
@@ -1178,54 +743,67 @@ text \<open>
 \<close>
 
 lemma CleanQ_Set_deq_n_x_ndst1 :
-  assumes I_holds : "CleanQ_Set_Invariants K rb"  and  X_owned: "\<forall>b \<in> B. b \<in> TYX rb"
-    shows "\<forall> b \<in> B. b \<notin> SY (CleanQ_Set_deq_n_x B rb)"
-  unfolding CleanQ_Set_deq_n_x_def using I_holds X_owned by auto
+assumes I_holds : "CleanQ_Set_Invariants K rb"  and  X_owned: "\<forall>b \<in> B. b \<in> TYX rb"
+  shows "\<forall> b \<in> B. b \<notin> SY (CleanQ_Set_deq_n_x B rb)"
+  using assms unfolding CleanQ_Set_deq_n_x_def CleanQ_Set_Invariants_simp by(auto)
 
 lemma CleanQ_Set_deq_n_x_ndst2 :
-  assumes I_holds : "CleanQ_Set_Invariants K rb"  and  X_owned: "\<forall>b \<in> B. b \<in> TYX rb"
-    shows "\<forall> b \<in> B. b \<notin> TXY (CleanQ_Set_deq_n_x B rb)"
-  unfolding CleanQ_Set_deq_n_x_def using I_holds X_owned by auto
+assumes I_holds : "CleanQ_Set_Invariants K rb"  and  X_owned: "\<forall>b \<in> B. b \<in> TYX rb"
+  shows "\<forall> b \<in> B. b \<notin> TXY (CleanQ_Set_deq_n_x B rb)"
+  using assms unfolding CleanQ_Set_deq_n_x_def CleanQ_Set_Invariants_simp by(auto)
 
 lemma CleanQ_Set_deq_n_x_ndst3 :
-  assumes I_holds : "CleanQ_Set_Invariants K rb"  and  X_owned: "\<forall>b \<in> B. b \<in> TYX rb"
-    shows "\<forall> b \<in> B. b \<notin> TYX (CleanQ_Set_deq_n_x B rb)"
-  unfolding CleanQ_Set_deq_n_x_def using I_holds X_owned by auto
+assumes I_holds : "CleanQ_Set_Invariants K rb"  and  X_owned: "\<forall>b \<in> B. b \<in> TYX rb"
+  shows "\<forall> b \<in> B. b \<notin> TYX (CleanQ_Set_deq_n_x B rb)"
+  using assms unfolding CleanQ_Set_deq_n_x_def CleanQ_Set_Invariants_simp by(auto)
 
 lemma CleanQ_Set_deq_n_y_ndst1 :
-  assumes I_holds : "CleanQ_Set_Invariants K rb"  and  Y_owned: "\<forall>b \<in> B. b \<in> TXY rb"
-    shows "\<forall> b \<in> B. b \<notin> SX (CleanQ_Set_deq_n_y B rb)"
-  unfolding CleanQ_Set_deq_n_y_def using I_holds Y_owned by auto
+assumes I_holds : "CleanQ_Set_Invariants K rb"  and  Y_owned: "\<forall>b \<in> B. b \<in> TXY rb"
+  shows "\<forall> b \<in> B. b \<notin> SX (CleanQ_Set_deq_n_y B rb)"
+  using assms unfolding CleanQ_Set_deq_n_y_def CleanQ_Set_Invariants_simp by(auto)
 
 lemma CleanQ_Set_deq_n_y_ndst2 :
-  assumes I_holds : "CleanQ_Set_Invariants K rb"  and  Y_owned: "\<forall>b \<in> B. b \<in> TXY rb"
-    shows "\<forall> b \<in> B. b \<notin> TXY (CleanQ_Set_deq_n_y B rb)"
-  unfolding CleanQ_Set_deq_n_y_def using I_holds Y_owned by auto
+assumes I_holds : "CleanQ_Set_Invariants K rb"  and  Y_owned: "\<forall>b \<in> B. b \<in> TXY rb"
+  shows "\<forall> b \<in> B. b \<notin> TXY (CleanQ_Set_deq_n_y B rb)"
+  using assms unfolding CleanQ_Set_deq_n_y_def CleanQ_Set_Invariants_simp by(auto)
 
 lemma CleanQ_Set_deq_n_y_ndst3 :
-  assumes I_holds : "CleanQ_Set_Invariants K rb"  and  Y_owned: "\<forall>b \<in> B. b \<in> TXY rb"
-    shows "\<forall> b \<in> B. b \<notin> TYX (CleanQ_Set_deq_n_y B rb)"
-  unfolding CleanQ_Set_deq_n_y_def using I_holds Y_owned by auto
+assumes I_holds : "CleanQ_Set_Invariants K rb"  and  Y_owned: "\<forall>b \<in> B. b \<in> TXY rb"
+  shows "\<forall> b \<in> B. b \<notin> TYX (CleanQ_Set_deq_n_y B rb)"
+  using assms unfolding CleanQ_Set_deq_n_y_def CleanQ_Set_Invariants_simp by(auto)
 
 text \<open>
   Finally, combining the lemmas above to obtain the result lemma of the operation.
 \<close>
 
 lemma CleanQ_Set_deq_n_x_result :
-  assumes I_holds : "CleanQ_Set_Invariants K rb"  and  YX_owned: "\<forall>b \<in> B. b \<in> TYX rb"
-      and CQ: "rb' = CleanQ_Set_deq_n_x B rb"
+assumes I_holds : "CleanQ_Set_Invariants K rb"  and  YX_owned: "\<forall>b \<in> B. b \<in> TYX rb"
+    and CQ: "rb' = CleanQ_Set_deq_n_x B rb"
     shows "\<forall>b \<in> B. b \<in> SX rb' \<and>  b \<notin> SY rb' \<and> b \<notin> TXY rb' \<and> b \<notin> TYX rb'"
   using assms
   by (simp add: CleanQ_Set_deq_n_x_dst CleanQ_Set_deq_n_x_ndst1 CleanQ_Set_deq_n_x_ndst2 
                 CleanQ_Set_deq_n_x_ndst3)
 
 lemma CleanQ_Set_deq_n_y_result :
-  assumes I_holds : "CleanQ_Set_Invariants K rb"  and  XY_owned: "\<forall>b \<in> B. b \<in> TXY rb"
-      and CQ: "rb' = CleanQ_Set_deq_n_y B rb"
-    shows "\<forall>b \<in> B. b \<in> SY rb' \<and>  b \<notin> SX rb' \<and> b \<notin> TXY rb' \<and> b \<notin> TYX rb'"
+assumes I_holds : "CleanQ_Set_Invariants K rb"  and  XY_owned: "\<forall>b \<in> B. b \<in> TXY rb"
+    and CQ: "rb' = CleanQ_Set_deq_n_y B rb"
+  shows "\<forall>b \<in> B. b \<in> SY rb' \<and>  b \<notin> SX rb' \<and> b \<notin> TXY rb' \<and> b \<notin> TYX rb'"
   using assms
   by (simp add: CleanQ_Set_deq_n_y_dst CleanQ_Set_deq_n_y_ndst1 CleanQ_Set_deq_n_y_ndst2 
                 CleanQ_Set_deq_n_y_ndst3)
+
+
+
+(* ------------------------------------------------------------------------------------ *)
+subsubsection \<open>Lemmas Summaries\<close>
+(* ------------------------------------------------------------------------------------ *)
+
+text \<open>
+  We define a few lemmas and lemma groups which simplify the proofs
+\<close>
+
+lemmas CleanQ_Set_ops_n = CleanQ_Set_deq_n_x_def CleanQ_Set_deq_n_y_def 
+                          CleanQ_Set_enq_n_x_def CleanQ_Set_enq_n_y_def
 
 
 (* ==================================================================================== *)
@@ -1260,9 +838,26 @@ lemma CleanQ_Set_enq_y_preserves_invariants :
       \<lbrace> CleanQ_Set_Invariants K \<acute>SetRB \<rbrace>"
   by(vcg, simp only: CleanQ_Set_enq_y_Invariants)
 
+text \<open>
+  The same applies for the multi-step \verb+eneuque_n+ operation.
+\<close>
+
+lemma CleanQ_Set_enq_n_x_preserves_invariants : 
+  "\<Gamma>\<turnstile> \<lbrace> rb' = \<acute>SetRB \<and> CleanQ_Set_Invariants K \<acute>SetRB \<and> (\<forall>b \<in> B. b \<in> (SX \<acute>SetRB)) \<rbrace> 
+        \<acute>SetRB :== (CleanQ_Set_enq_n_x B \<acute>SetRB) 
+      \<lbrace> CleanQ_Set_Invariants K \<acute>SetRB \<rbrace>"
+  apply(vcg) using CleanQ_Set_enq_n_x_Invariants by blast
+
+lemma CleanQ_Set_enq_n_y_preserves_invariants : 
+  "\<Gamma>\<turnstile> \<lbrace> rb' = \<acute>SetRB \<and> CleanQ_Set_Invariants K \<acute>SetRB \<and> (\<forall>b \<in> B. b \<in> (SY \<acute>SetRB)) \<rbrace> 
+        \<acute>SetRB :== (CleanQ_Set_enq_n_y B \<acute>SetRB) 
+      \<lbrace> CleanQ_Set_Invariants K \<acute>SetRB \<rbrace>"
+  apply(vcg) using CleanQ_Set_enq_n_y_Invariants by blast
+
+
 
 text \<open>
-  The enqueue operation effectively happens in two steps. The buffer element is removed
+  The enqueue operation  happens in two steps. The buffer element is removed
   from one set and added to a new set. We can express this as two sequential operations
   in the next lemma, where we show that the invariant is still preserved and that 
   the outcome is the same, as with the definition above.
@@ -1273,18 +868,21 @@ lemma CleanQ_Set_enq_x_two_step:
         \<acute>SetRB :== \<acute>SetRB \<lparr> SX := (SX \<acute>SetRB) - {b} \<rparr> ;;
         \<acute>SetRB :== \<acute>SetRB \<lparr> TXY := (TXY \<acute>SetRB) \<union> {b} \<rparr>  
       \<lbrace> \<acute>SetRB = CleanQ_Set_enq_x b rb' \<and> CleanQ_Set_Invariants K \<acute>SetRB \<rbrace>"
-  by(vcg, simp add: CleanQ_Set_enq_x_def, auto)
+  by(vcg, auto simp:CleanQ_Set_Invariants_simp CleanQ_Set_enq_x_def)
+  
 
 lemma CleanQ_Set_enq_y_two_step:
   "\<Gamma>\<turnstile> \<lbrace> rb' = \<acute>SetRB \<and> CleanQ_Set_Invariants K \<acute>SetRB \<and> b \<in> SY \<acute>SetRB \<rbrace>
         \<acute>SetRB :== \<acute>SetRB \<lparr> SY := (SY \<acute>SetRB) - {b} \<rparr> ;;
         \<acute>SetRB :== \<acute>SetRB \<lparr> TYX := (TYX \<acute>SetRB) \<union> {b} \<rparr>  
       \<lbrace> \<acute>SetRB = CleanQ_Set_enq_y b rb' \<and> CleanQ_Set_Invariants K \<acute>SetRB \<rbrace>"
-  by(vcg, simp add: CleanQ_Set_enq_y_def, auto)
+  by(vcg, auto simp:CleanQ_Set_Invariants_simp CleanQ_Set_enq_y_def)
+  
+
 
 text \<open>
   Next we can define this conditionally, where we only execute the enqueue operation, 
-  when we are owning the buffer
+  when we are owning the buffer. 
 \<close>
 
 lemma CleanQ_Set_enq_x_conditional :
@@ -1292,34 +890,21 @@ lemma CleanQ_Set_enq_x_conditional :
          IF b \<in> SX \<acute>SetRB THEN 
           \<acute>SetRB :== (CleanQ_Set_enq_x b \<acute>SetRB) 
          FI 
-      \<lbrace> CleanQ_Set_Invariants K \<acute>SetRB \<rbrace>" 
-  by (vcg, meson CleanQ_Set_enq_x_Invariants)
+      \<lbrace> CleanQ_Set_Invariants K \<acute>SetRB \<and> b \<notin> (SX \<acute>SetRB) \<rbrace>" 
+  by(vcg, auto simp:CleanQ_Set_enq_x_Invariants CleanQ_Set_enq_x_def 
+                    CleanQ_Set_Invariants_simp)
+  
 
 lemma CleanQ_Set_enq_y_conditional :
   "\<Gamma>\<turnstile> \<lbrace> CleanQ_Set_Invariants K \<acute>SetRB \<rbrace> 
          IF b \<in> SY \<acute>SetRB THEN 
           \<acute>SetRB :== (CleanQ_Set_enq_y b \<acute>SetRB) 
          FI 
-      \<lbrace> CleanQ_Set_Invariants K \<acute>SetRB \<rbrace>" 
-  by (vcg, meson CleanQ_Set_enq_y_Invariants)
+      \<lbrace> CleanQ_Set_Invariants K \<acute>SetRB \<and>  b \<notin> (SY \<acute>SetRB) \<rbrace>" 
+  by(vcg, auto simp:CleanQ_Set_enq_y_Invariants CleanQ_Set_enq_y_def 
+                    CleanQ_Set_Invariants_simp)
 
 
-(*
-
-can we define a procedure of this, which can be called by a thread?
-probably with a guard.
-
-procedures 
-  EnqX (S|R) = "IF (SX \<acute>S) \<noteq>  \<emptyset> THEN
-                ... pick a b
-                 \<acute>SetRB :== (CleanQ_Set_enq_x b \<acute>SetRB) 
-                FI"
-
-  EnqX (S|R) = "SWITCH (SX \<acute>S)
-                    {{b} \<union> _} \<Rightarrow> \<acute>R :== (CleanQ_Set_enq_x b \<acute>S) 
-                  | {} \<Rightarrow> \<acute>R = \<acute>S
-               END"
-*)
 
 (* ------------------------------------------------------------------------------------ *)
 subsubsection \<open>Dequeue Operation\<close>
@@ -1345,6 +930,23 @@ lemma CleanQ_Set_deq_y_preserves_invariants:
 
 
 text \<open>
+  The same applies for the multi-step \verb+eneuque_n+ operation.
+\<close>
+
+lemma CleanQ_Set_deq_n_x_preserves_invariants: 
+  "\<Gamma>\<turnstile> \<lbrace> rb' = \<acute>SetRB \<and> CleanQ_Set_Invariants K \<acute>SetRB \<and> (\<forall> b \<in> B. b \<in> TYX \<acute>SetRB) \<rbrace> 
+        \<acute>SetRB :== (CleanQ_Set_deq_n_x B \<acute>SetRB) 
+      \<lbrace> CleanQ_Set_Invariants K \<acute>SetRB \<rbrace>"
+  apply(vcg) using CleanQ_Set_deq_n_x_Invariants by blast
+
+lemma CleanQ_Set_deq_n_y_preserves_invariants: 
+  "\<Gamma>\<turnstile> \<lbrace> rb' = \<acute>SetRB \<and> CleanQ_Set_Invariants K \<acute>SetRB \<and> (\<forall> b \<in> B. b \<in> TXY \<acute>SetRB) \<rbrace> 
+        \<acute>SetRB :== (CleanQ_Set_deq_n_y B \<acute>SetRB) 
+      \<lbrace> CleanQ_Set_Invariants K \<acute>SetRB \<rbrace>"
+  apply(vcg) using CleanQ_Set_deq_n_y_Invariants by blast
+
+
+text \<open>
   The dequeue operation effectively happens in two steps. The buffer element is removed
   from one set and added to a new set. We can express this as two sequential operations
   in the next lemma, where we show that the invariant is still preserved and that 
@@ -1356,14 +958,14 @@ lemma CleanQ_Set_deq_x_two_step:
         \<acute>SetRB :== \<acute>SetRB \<lparr> TYX := (TYX \<acute>SetRB) - {b} \<rparr> ;;
         \<acute>SetRB :== \<acute>SetRB \<lparr> SX := (SX \<acute>SetRB) \<union> {b} \<rparr>  
       \<lbrace> \<acute>SetRB = CleanQ_Set_deq_x b rb' \<and> CleanQ_Set_Invariants K \<acute>SetRB \<rbrace>"
-  by(vcg, simp add: CleanQ_Set_deq_x_def, auto)
+  by(vcg, simp add: CleanQ_Set_deq_x_def CleanQ_Set_Invariants_simp, auto)
 
 lemma CleanQ_Set_deq_y_two_step:
   "\<Gamma>\<turnstile> \<lbrace> rb' = \<acute>SetRB \<and> CleanQ_Set_Invariants K \<acute>SetRB \<and> b \<in> TXY \<acute>SetRB \<rbrace>
         \<acute>SetRB :== \<acute>SetRB \<lparr> TXY := (TXY \<acute>SetRB) - {b} \<rparr> ;;
         \<acute>SetRB :== \<acute>SetRB \<lparr> SY := (SY \<acute>SetRB) \<union> {b} \<rparr>  
       \<lbrace> \<acute>SetRB = CleanQ_Set_deq_y b rb' \<and> CleanQ_Set_Invariants K \<acute>SetRB \<rbrace>"
-  by(vcg, simp add: CleanQ_Set_deq_y_def, auto)
+  by(vcg, simp add: CleanQ_Set_deq_y_def CleanQ_Set_Invariants_simp, auto)
 
 
 text \<open>
@@ -1406,38 +1008,584 @@ lemma CleanQ_Set_ops_combine :
         \<acute>SetRB :== (CleanQ_Set_enq_y b \<acute>SetRB) ;;
         \<acute>SetRB :== (CleanQ_Set_deq_x b \<acute>SetRB) 
       \<lbrace> CleanQ_Set_Invariants K \<acute>SetRB \<and> rb = \<acute>SetRB \<and> b \<in> SX \<acute>SetRB \<rbrace>" 
-proof(vcg)
-  have EQ: "\<And> RB. CleanQ_Set_Invariants K RB \<Longrightarrow> b \<in> SX RB \<Longrightarrow> (CleanQ_Set_deq_x b
-             (CleanQ_Set_enq_y b
-               (CleanQ_Set_deq_y b
-                 (CleanQ_Set_enq_x b RB)))) = RB"
-    unfolding CleanQ_Set_deq_x_def CleanQ_Set_enq_x_def CleanQ_Set_deq_y_def 
-              CleanQ_Set_enq_y_def
-    apply(simp) 
-    using insert_absorb by fastforce
+  apply(vcg, auto simp:CleanQ_Set_ops CleanQ_Set_Invariants_simp)
+  using insert_absorb by fastforce
+  
 
-  from EQ  show "\<And>RB. CleanQ_Set_Invariants K RB \<Longrightarrow>
-          b \<in> SX RB \<Longrightarrow>
-          CleanQ_Set_Invariants K
-           (CleanQ_Set_deq_x b
-             (CleanQ_Set_enq_y b
-               (CleanQ_Set_deq_y b
-                 (CleanQ_Set_enq_x b RB)))) \<and>
-          RB =
-          CleanQ_Set_deq_x b
-           (CleanQ_Set_enq_y b
-             (CleanQ_Set_deq_y b (CleanQ_Set_enq_x b RB))) \<and>
-          b \<in> SX (CleanQ_Set_deq_x b
-                    (CleanQ_Set_enq_y b
-                      (CleanQ_Set_deq_y b
-                        (CleanQ_Set_enq_x b RB))))"
-    by(auto)
+
+  
+(* ==================================================================================== *)
+subsection \<open>Strong and Weak Frame Conditions\<close>
+(* ==================================================================================== *)
+
+text \<open>
+  We now define the strong and weak frame conditions for the CleanQ Set model. Those are
+  used in the concurrency proofs. They define the set of operations the other side can
+  do to the state of the queue system. 
+\<close>
+
+
+(* ------------------------------------------------------------------------------------ *)
+subsubsection \<open>Strong Frame Condition\<close>
+(* ------------------------------------------------------------------------------------ *)
+
+text \<open>
+  The strong frame condition as we currently have it can be defined as shown below. The 
+  essence of it is that no set changes which is not specifically defined to change.
+\<close>
+
+type_synonym 'a tuple = "'a set \<times> 'a set \<times> 'a set \<times> 'a set"
+
+fun CleanQ_Set_Frame_Strong :: "'a tuple \<Rightarrow>'a tuple \<Rightarrow> bool"
+  where "CleanQ_Set_Frame_Strong (sx',txy',sy',tyx') (sx,txy,sy,tyx) \<longleftrightarrow> 
+                                          sx' = sx \<and> txy' = txy \<and> sy' = sy \<and> tyx' = tyx"
+
+text \<open>
+  For the concurrent case, we can not assume that the sets we do not explicitly modify by 
+  an operation do not change and for this we have to weaken the frame condition that 
+  e.g. when enqueueing from X the sets TXY, SY and TYX might change through actions of Y.
+\<close>
+definition  CleanQ_Set_Frame_Weak_x :: 
+    "'a CleanQ_Set_State \<Rightarrow> 'a CleanQ_Set_State \<Rightarrow> 'a set \<Rightarrow> 'a set \<Rightarrow> bool"
+    where "CleanQ_Set_Frame_Weak_x st' st dtxy dsy  \<longleftrightarrow> 
+            SX st = SX st' \<and> SY st \<union> dsy = SY st'\<union> dtxy \<and>
+            TXY st \<union> dtxy  = TXY st' \<and> TYX st = TYX st' \<union> dsy \<and>
+            dsy \<inter> (SY st) = {} \<and> dtxy \<inter> TXY st = {} \<and> dsy \<inter> TXY st = {}"
+
+definition  CleanQ_Set_Frame_Weak_y :: 
+    "'a CleanQ_Set_State \<Rightarrow> 'a CleanQ_Set_State \<Rightarrow> 'a set \<Rightarrow> 'a set \<Rightarrow> bool"
+    where "CleanQ_Set_Frame_Weak_y st' st dtyx dsx  \<longleftrightarrow> 
+            SY st = SY st' \<and> SX st \<union> dsx = SX st'\<union> dtyx \<and>
+            TYX st \<union> dtyx  = TYX st' \<and> TXY st = TXY st' \<union> dsx \<and>
+            dsx \<inter> (SX st) = {} \<and> dtyx \<inter> TYX st = {} \<and> dsx \<inter> TYX st = {}  "
+
+
+text \<open>
+  We can now show, that enqueue  and dequeue operations fulfil the weak frame condition.
+\<close>
+
+lemma CleanQ_Set_Frame_Weak_x_enq:
+  assumes I: "CleanQ_Set_Invariants K st'"  and  owns: "b \<in> SY st'"
+    shows "CleanQ_Set_Frame_Weak_x st' (CleanQ_Set_enq_y b st') {} {b}"
+  using assms unfolding CleanQ_Set_Frame_Weak_x_def CleanQ_Set_enq_y_def 
+  by(auto simp:CleanQ_Set_Invariants_simp)
+
+lemma CleanQ_Set_Frame_Weak_x_deq:
+  assumes I: "CleanQ_Set_Invariants K st'"  and  owns: "b \<in> TXY st'"
+    shows "CleanQ_Set_Frame_Weak_x st' (CleanQ_Set_deq_y b st') {b} {}"
+  using assms unfolding CleanQ_Set_Frame_Weak_x_def CleanQ_Set_deq_y_def  by(auto)
+
+lemma CleanQ_Set_Frame_Weak_y_enq:
+  assumes I: "CleanQ_Set_Invariants K st'"  and  owns: "b \<in> SX st'"
+    shows "CleanQ_Set_Frame_Weak_y st' (CleanQ_Set_enq_x b st') {} {b}"
+  using assms unfolding CleanQ_Set_Frame_Weak_y_def CleanQ_Set_enq_x_def 
+  by(auto simp:CleanQ_Set_Invariants_simp)
+
+lemma CleanQ_Set_Frame_Weak_y_deq:
+  assumes I: "CleanQ_Set_Invariants K st'"  and  owns: "b \<in> TYX st'"
+    shows "CleanQ_Set_Frame_Weak_y st' (CleanQ_Set_deq_x b st') {b} {}"
+  using assms unfolding CleanQ_Set_Frame_Weak_y_def CleanQ_Set_deq_x_def  by(auto)
+
+text \<open>
+  The weak frame conditions imply where the sets must come from. 
+\<close>
+
+lemma  CleanQ_Set_Frame_Weak_y_owns1:
+  "CleanQ_Set_Frame_Weak_y st' st {} B \<Longrightarrow> B \<subseteq> SX st'"
+  unfolding CleanQ_Set_Frame_Weak_y_def by(auto)
+
+lemma  CleanQ_Set_Frame_Weak_y_owns2:
+  "CleanQ_Set_Frame_Weak_y st' st A {} \<Longrightarrow> A \<subseteq> TYX st'"
+  unfolding CleanQ_Set_Frame_Weak_y_def by(auto)
+
+lemma  CleanQ_Set_Frame_Weak_x_owns1:
+  "CleanQ_Set_Frame_Weak_x st' st {} B \<Longrightarrow> B \<subseteq> SY st'"
+  unfolding CleanQ_Set_Frame_Weak_x_def by(auto)
+
+lemma  CleanQ_Set_Frame_Weak_x_owns2:
+  "CleanQ_Set_Frame_Weak_x st' st A {} \<Longrightarrow> A \<subseteq> TXY st'"
+  unfolding CleanQ_Set_Frame_Weak_x_def by(auto)
+
+
+text \<open>The weak frame condition for an \verb+enqueue+ or \verb+dequeue+ preserves I1. \<close>
+
+lemma CleanQ_Set_enq_x_I1_weak:
+assumes I: "CleanQ_Set_Invariants K st'" 
+   and frame: "CleanQ_Set_Frame_Weak_y st' st {} {b}"
+ shows "I1 st K"
+  using assms unfolding I1_def CleanQ_Set_Frame_Weak_y_def CleanQ_Set_Invariants_def
+  by(auto simp:CleanQ_Set_Invariants_simp)
+  
+lemma CleanQ_Set_enq_y_I1_weak:
+assumes I: "CleanQ_Set_Invariants K st'" 
+   and frame: "CleanQ_Set_Frame_Weak_x st' st {} {b}"
+ shows "I1 st K"
+  using assms unfolding I1_def CleanQ_Set_Frame_Weak_x_def CleanQ_Set_Invariants_def
+  by(auto simp:CleanQ_Set_Invariants_simp)
+
+lemma CleanQ_Set_deq_x_I1_weak:
+assumes I: "CleanQ_Set_Invariants K st'" 
+   and frame: "CleanQ_Set_Frame_Weak_y st' st {b} {}"
+ shows "I1 st K"
+  using assms unfolding I1_def CleanQ_Set_Frame_Weak_y_def CleanQ_Set_Invariants_def
+  by(auto simp:CleanQ_Set_Invariants_simp)
+
+lemma CleanQ_Set_deq_y_I1_weak:
+assumes I: "CleanQ_Set_Invariants K st'"
+   and frame: "CleanQ_Set_Frame_Weak_x st' st {b} {}"
+ shows "I1 st K"
+  using assms unfolding I1_def CleanQ_Set_Frame_Weak_x_def CleanQ_Set_Invariants_def
+  by(auto simp:CleanQ_Set_Invariants_simp)
+
+text \<open>The weak frame condition for an \verb+enqueue+ or \verb+dequeue+ preserves I2. \<close>
+
+lemma CleanQ_Set_enq_x_I2_weak:
+assumes I: "CleanQ_Set_Invariants K st'" 
+   and frame: "CleanQ_Set_Frame_Weak_y st' st {} {b}"
+ shows "I2 st"
+  using assms unfolding I2_def CleanQ_Set_Frame_Weak_y_def CleanQ_Set_Invariants_def
+  by(auto)  
+
+lemma CleanQ_Set_deq_x_I2_weak:
+assumes I: "CleanQ_Set_Invariants K st'" 
+   and frame: "CleanQ_Set_Frame_Weak_y st' st {b} {}" 
+ shows "I2 st"
+  using assms unfolding I2_def CleanQ_Set_Frame_Weak_y_def CleanQ_Set_Invariants_def
+  by(auto)  
+
+lemma CleanQ_Set_enq_y_I2_weak:
+assumes I: "CleanQ_Set_Invariants K st'" 
+   and frame: "CleanQ_Set_Frame_Weak_x st' st {} {b}"
+ shows "I2 st"
+  using assms unfolding I2_def CleanQ_Set_Frame_Weak_x_def CleanQ_Set_Invariants_def
+  by(auto)  
+
+lemma CleanQ_Set_deq_y_I2_weak:
+assumes I: "CleanQ_Set_Invariants K st'" 
+   and frame: "CleanQ_Set_Frame_Weak_x st' st {b} {}" 
+ shows "I2 st"
+  using assms unfolding I2_def CleanQ_Set_Frame_Weak_x_def CleanQ_Set_Invariants_def
+  by(auto)  
+
+
+
+(* ------------------------------------------------------------------------------------ *)
+subsubsection \<open>Generic Frame Conditions\<close>
+(* ------------------------------------------------------------------------------------ *)
+
+text \<open>
+  Generically, the frame condition is the equivalence of sets, that are not being talked
+  about.
+\<close>
+
+fun frame_strong ::
+  "'a \<times> 'b \<times> 'c \<times> 'd \<Rightarrow>'a \<times> 'b \<times> 'c \<times> 'd \<Rightarrow> bool"
+  where "frame_strong (A',B',C',D') (A,B,C,D) \<longleftrightarrow> A' = A \<and> B' = B \<and> C' = C \<and> D' = D"
+
+
+text \<open>@{term D} is in its initial state, but elements may move from @{term A} to @{term B}
+  and from @{term B} to @{term C}.\<close>
+
+fun frame_weak ::
+  "'a set \<times> 'a set \<times> 'a set \<times> 'a set \<Rightarrow> 'a set \<times> 'a set \<times> 'a set \<times> 'a set \<Rightarrow> bool"
+  where "frame_weak (A',B',C',D') (A,B,C,D) \<longleftrightarrow>  D' = D \<and> (\<exists>\<Delta>AB \<Delta>BC.
+    A \<union> \<Delta>AB = A'\<and>        
+    B \<union> \<Delta>BC = B' \<union> \<Delta>AB \<and>    
+    C = C' \<union> \<Delta>BC \<and>    
+    A \<inter> \<Delta>BC = {} \<and>
+    A \<inter> \<Delta>AB = {} \<and>      
+    B \<inter> \<Delta>BC = {} )"
+
+
+text \<open>
+  We can show equivalent to the frame conditions above
+\<close>
+lemma CleanQ_Set_frame_weak_equiv_x:
+  "frame_weak (TXY st', SY st', TYX st', SX st' ) (TXY st, SY st, TYX st, SX st)
+                              \<longleftrightarrow> (\<exists>\<Delta>AB \<Delta>BC. CleanQ_Set_Frame_Weak_x st' st \<Delta>AB \<Delta>BC)"
+  unfolding frame_weak.simps CleanQ_Set_Frame_Weak_x_def 
+  by (metis Int_commute)
+  
+
+lemma CleanQ_Set_frame_weak_equiv_y:
+  "frame_weak (TYX st', SX st', TXY st', SY st' ) (TYX st, SX st, TXY st, SY st) 
+                             \<longleftrightarrow> (\<exists>\<Delta>AB \<Delta>BC. CleanQ_Set_Frame_Weak_y st' st \<Delta>AB \<Delta>BC)"
+  unfolding frame_weak.simps CleanQ_Set_Frame_Weak_y_def
+  by (metis Int_commute)
+
+text \<open>
+  As a first step we have to show that the strong frame condition implies the weak one.
+\<close>
+
+lemma frame_s_w:
+  "frame_strong (A',B',C',D') (A,B,C,D) \<Longrightarrow> frame_weak (A',B',C',D') (A,B,C,D)"
+  unfolding frame_strong.simps frame_weak.simps by(blast)
+
+
+text \<open>The weak frame condition for an enqueue from @{term D} into @{term A} preserves
+  invariant 1.\<close>
+
+lemma CleanQ_Set_enq_x_I1_weak2:
+  fixes st st' K b
+  assumes I: "CleanQ_Set_Invariants K st'"
+      and rb: "st = CleanQ_Set_enq b st'"
+      and frame: "frame_weak (TXY st' \<union> {b},SY st', TYX st', SX st' - {b}) (TXY st, SY st, TYX st, SX st)"
+      and owns: "b \<in> SX st'"
+    shows "I1 st K"
+  using assms subst unfolding frame_weak.simps I1_def
+  by (smt CleanQ_Set_Invariants_def I1_def Un_insert_right insert_Diff 
+          sup_aci(3) sup_assoc sup_bot.comm_neutral)
+
+lemma CleanQ_Set_enq_y_I1_weak2:
+  fixes st st' K b
+  assumes I: "CleanQ_Set_Invariants K st'"
+      and rb: "st = CleanQ_Set_enq b st'"
+      and frame: "frame_weak (TYX st' \<union> {b},SX st', TXY st', SY st' - {b}) (TYX st, SX st, TXY st, SY st)"
+      and owns: "b \<in> SY st'"
+    shows "I1 st K"
+  using assms subst unfolding frame_weak.simps I1_def
+  by (smt CleanQ_Set_Invariants_def I1_def Un_insert_right insert_Diff sup_aci(3)
+          sup_assoc sup_bot.comm_neutral)
+
+lemma CleanQ_Set_enq_x_I2_weak2:
+  fixes st st' K b
+  assumes I: "CleanQ_Set_Invariants K st'"
+      and rb: "st = CleanQ_Set_enq b st'"
+      and frame: "frame_weak (TXY st' \<union> {b},SY st', TYX st', SX st' - {b}) (TXY st, SY st, TYX st, SX st)"
+      and owns: "b \<in> SX st'"
+    shows "I2 st"
+proof(unfold I2_def, intro conjI)
+  from frame obtain \<Delta>AB \<Delta>BC where
+    fA: "(TXY st' \<union> {b}) = \<Delta>AB \<union> TXY st" and
+    fB: "SY st' \<union> \<Delta>AB = \<Delta>BC \<union> SY st" and
+    fC: "TYX st' \<union> \<Delta>BC = TYX st" and
+    fD: "SX st' - {b} = SX st" and
+    dAB: "TXY st \<inter> \<Delta>AB = {}" and
+    dAC: "TXY st \<inter> \<Delta>BC = {}" and
+    dBC: "SY st \<inter> \<Delta>BC = {}"
+    by (metis (no_types, lifting) frame_weak.simps sup.commute)
+
+  from fA have ss_\<Delta>AB: "\<Delta>AB \<subseteq> TXY st' \<union> {b}" by(auto)
+  with fB have ss_\<Delta>BC: "\<Delta>BC \<subseteq> TXY st' \<union> SY st' \<union> {b}" by(auto)
+
+  from fA have ss_A: "TXY st \<subseteq> TXY st' \<union> {b}" by(auto)
+  from fB ss_\<Delta>AB have ss_B: "SY st \<subseteq> TXY st' \<union> SY st' \<union> {b}" by(auto)
+  from fC ss_\<Delta>BC have ss_C: "TYX st \<subseteq> TXY st' \<union> SY st' \<union> TYX st' \<union> {b}" by(auto)
+
+  from I ss_A show "SX st \<inter> TXY st = {}" by(unfold fD[symmetric], auto simp:CleanQ_Set_Invariants_simp)
+  from I ss_B show "SX st \<inter> SY st = {}" by(unfold fD[symmetric], auto simp:CleanQ_Set_Invariants_simp)
+  from I ss_C show "SX st \<inter> TYX st = {}" by(unfold fD[symmetric], auto simp:CleanQ_Set_Invariants_simp)
+
+  from fC have "SY st \<inter> TYX st = SY st \<inter> (TYX st' \<union> \<Delta>BC)" by(simp)
+  also have "... = (SY st \<inter> TYX st') \<union> (SY st \<inter> \<Delta>BC)" by(auto)
+  also {
+    from ss_B have "SY st \<inter> TYX st' \<subseteq> (TXY st' \<union> SY st' \<union> {b}) \<inter> TYX st'" by(auto)
+    also from I owns have "... = {}" by(auto simp:CleanQ_Set_Invariants_simp)
+    finally have "(SY st \<inter> TYX st') \<union> (SY st \<inter> \<Delta>BC) = SY st \<inter> \<Delta>BC" by(simp)
+  }
+  txt \<open>@{term "SY st \<inter> \<Delta>BC = {}"} is essential\<close>
+  finally have "SY st \<inter> TYX st = SY st \<inter> \<Delta>BC" .
+  with dBC show "SY st \<inter> TYX st = {}" by(simp)
+
+  from fC have "TXY st \<inter> TYX st = TXY st \<inter> (TYX st' \<union> \<Delta>BC)" by(simp)
+  also have "... = (TXY st \<inter> TYX st') \<union> (TXY st \<inter> \<Delta>BC)" by(auto)
+  also {
+    from ss_A have "TXY st \<inter> TYX st' \<subseteq> (TXY st' \<union> {b}) \<inter> TYX st'" by(auto)
+    also from I owns have "... = {}" by(auto simp:CleanQ_Set_Invariants_simp)
+    finally have "(TXY st \<inter> TYX st') \<union> (TXY st \<inter> \<Delta>BC) = TXY st \<inter> \<Delta>BC" by(simp)
+  }
+  txt \<open>@{term "TXY st \<inter> \<Delta>BC = {}"} is essential\<close>
+  finally have "TXY st \<inter> TYX st = TXY st \<inter> \<Delta>BC" .
+  with dAC show "TXY st \<inter> TYX st = {}" by(simp add:CleanQ_Set_Invariants_simp)
+
+  from fB have "TXY st \<inter> (\<Delta>BC \<union> SY st) = TXY st \<inter> (SY st' \<union> \<Delta>AB)" by(simp)
+  also have "... = (TXY st \<inter> SY st') \<union> (TXY st \<inter> \<Delta>AB)" by(auto)
+  also {
+    from ss_A have "TXY st \<inter> SY st' \<subseteq> (TXY st' \<union> {b}) \<inter> SY st'" by(auto)
+    also from I owns have "... = {}" by(auto simp:CleanQ_Set_Invariants_simp)
+    finally have "(TXY st \<inter> SY st') \<union> (TXY st \<inter> \<Delta>AB) = TXY st \<inter> \<Delta>AB" by(simp)
+  }
+  txt \<open>@{term "TXY st \<inter> \<Delta>AB = {}"} is essential, given @{term "TXY st \<inter> \<Delta>BC = {}"}.\<close>
+  finally have "TXY st \<inter> (\<Delta>BC \<union> SY st) = TXY st \<inter> \<Delta>AB" .
+  with dAB show "SY st \<inter> TXY st = {}" by auto
 qed
 
-  
-  
+lemma CleanQ_Set_enq_y_I2_weak2:
+  fixes st st' K b
+  assumes I: "CleanQ_Set_Invariants K st'"
+      and rb: "st = CleanQ_Set_enq b st'"
+      and frame: "frame_weak (TYX st' \<union> {b},SX st', TXY st', SY st' - {b}) (TYX st, SX st, TXY st, SY st)"
+      and owns: "b \<in> SY st'"
+    shows "I2 st"
+proof(unfold I2_def, intro conjI)
+  from frame obtain \<Delta>AB \<Delta>BC where
+    fA: "(TYX st' \<union> {b}) = \<Delta>AB \<union> TYX st" and
+    fB: "SX st' \<union> \<Delta>AB = \<Delta>BC \<union> SX st" and
+    fC: "TXY st' \<union> \<Delta>BC = TXY st" and
+    fD: "SY st' - {b} = SY st" and
+    dAB: "TYX st \<inter> \<Delta>AB = {}" and
+    dAC: "TYX st \<inter> \<Delta>BC = {}" and
+    dBC: "SX st \<inter> \<Delta>BC = {}"
+    by (metis (no_types, lifting) frame_weak.simps sup.commute)
+
+  from fA have ss_\<Delta>AB: "\<Delta>AB \<subseteq> TYX st' \<union> {b}" by(auto)
+  with fB have ss_\<Delta>BC: "\<Delta>BC \<subseteq> TYX st' \<union> SX st' \<union> {b}" by(auto)
+
+  from fA have ss_A: "TYX st \<subseteq> TYX st' \<union> {b}" by(auto)
+  from fB ss_\<Delta>AB have ss_B: "SX st \<subseteq> TYX st' \<union> SX st' \<union> {b}" by(auto)
+  from fC ss_\<Delta>BC have ss_C: "TXY st \<subseteq> TYX st' \<union> SX st' \<union> TXY st' \<union> {b}" by(auto)
+
+  from I ss_A show "SY st \<inter> TYX st = {}" by(unfold fD[symmetric], auto simp:CleanQ_Set_Invariants_simp)
+  from I ss_B show "SX st \<inter> SY st = {}" by(unfold fD[symmetric], auto simp:CleanQ_Set_Invariants_simp)
+  from I ss_C show "SY st \<inter> TXY st = {}" by(unfold fD[symmetric], auto simp:CleanQ_Set_Invariants_simp)
+
+  from fC have "SX st \<inter> TXY st = SX st \<inter> (TXY st' \<union> \<Delta>BC)" by(simp)
+  also have "... = (SX st \<inter> TXY st') \<union> (SX st \<inter> \<Delta>BC)" by(auto)
+  also {
+    from ss_B have "SX st \<inter> TXY st' \<subseteq> (TYX st' \<union> SX st' \<union> {b}) \<inter> TXY st'" by(auto)
+    also from I owns have "... = {}" by(auto simp:CleanQ_Set_Invariants_simp)
+    finally have "(SX st \<inter> TXY st') \<union> (SX st \<inter> \<Delta>BC) = SX st \<inter> \<Delta>BC" by(simp)
+  }
+  txt \<open>@{term "SX st \<inter> \<Delta>BC = {}"} is essential\<close>
+  finally have "SX st \<inter> TXY st = SX st \<inter> \<Delta>BC" .
+  with dBC show "SX st \<inter> TXY st = {}" by(simp)
+
+  from fC have "TYX st \<inter> TXY st = TYX st \<inter> (TXY st' \<union> \<Delta>BC)" by(simp)
+  also have "... = (TYX st \<inter> TXY st') \<union> (TYX st \<inter> \<Delta>BC)" by(auto)
+  also {
+    from ss_A have "TYX st \<inter> TXY st' \<subseteq> (TYX st' \<union> {b}) \<inter> TXY st'" by(auto)
+    also from I owns have "... = {}" by(auto simp:CleanQ_Set_Invariants_simp)
+    finally have "(TYX st \<inter> TXY st') \<union> (TYX st \<inter> \<Delta>BC) = TYX st \<inter> \<Delta>BC" by(simp)
+  }
+  txt \<open>@{term "TYX st \<inter> \<Delta>BC = {}"} is essential\<close>
+  finally have "TYX st \<inter> TXY st = TYX st \<inter> \<Delta>BC" .
+  with dAC show "TXY st \<inter> TYX st = {}" by(blast)
+
+  from fB have "TYX st \<inter> (\<Delta>BC \<union> SX st) = TYX st \<inter> (SX st' \<union> \<Delta>AB)" by(simp)
+  also have "... = (TYX st \<inter> SX st') \<union> (TYX st \<inter> \<Delta>AB)" by(auto)
+  also {
+    from ss_A have "TYX st \<inter> SX st' \<subseteq> (TYX st' \<union> {b}) \<inter> SX st'" by(auto)
+    also from I owns have "... = {}" by(auto simp:CleanQ_Set_Invariants_simp)
+    finally have "(TYX st \<inter> SX st') \<union> (TYX st \<inter> \<Delta>AB) = TYX st \<inter> \<Delta>AB" by(simp)
+  }
+  txt \<open>@{term "TYX st \<inter> \<Delta>AB = {}"} is essential, given @{term "TYX st \<inter> \<Delta>BC = {}"}.\<close>
+  finally have "TYX st \<inter> (\<Delta>BC \<union> SX st) = TYX st \<inter> \<Delta>AB" .
+  with dAB show "SX st \<inter> TYX st = {}" by auto
+qed
 
 
+
+
+
+
+lemma CleanQ_Set_enq_x_weak_Invariants :
+  fixes st st' K b
+  assumes I: "CleanQ_Set_Invariants K st'"
+      and rb: "st = CleanQ_Set_enq_x b st'"
+      and frame: "frame_weak (TXY st' \<union> {b},SY st', TYX st', SX st' - {b}) (TXY st, SY st, TYX st, SX st)"
+      and owns: "b \<in> SX st'"
+    shows "CleanQ_Set_Invariants K (CleanQ_Set_enq_x b st)"  
+  by (metis CleanQ_Set_State.ext_inject CleanQ_Set_State.surjective CleanQ_Set_enq_x_Invariants 
+      CleanQ_Set_enq_x_upd Diff_idemp I owns rb sup.right_idem)
+
+
+
+
+lemma CleanQ_Set_enq_y_weak_Invariants :
+  fixes st st' K b
+  assumes I: "CleanQ_Set_Invariants K st'"
+      and rb: "st = CleanQ_Set_enq_y b st'"
+      and frame: "frame_weak (TYX st' \<union> {b},SX st', TXY st', SY st' - {b}) (TYX st, SX st, TXY st, SY st)"
+      and owns: "b \<in> SY st'"
+    shows "CleanQ_Set_Invariants K (CleanQ_Set_enq_y b st)"  
+  by (metis CleanQ_Set_State.ext_inject CleanQ_Set_State.surjective CleanQ_Set_enq_y_Invariants 
+      CleanQ_Set_enq_y_upd Diff_idemp I owns rb sup.right_idem)
+
+
+
+(* ------------------------------------------------------------------------------------ *)
+subsubsection \<open>Dequeue Operation\<close>
+(* ------------------------------------------------------------------------------------ *)
+
+
+text \<open>
+  Similar to enqueue we also have to show the same for dequeue and the weak frame condition
+\<close>
+
+lemma CleanQ_Set_deq_x_weak_I1:
+  fixes st st' K b
+  assumes I: "CleanQ_Set_Invariants K st'"
+      and rb: "st = CleanQ_Set_deq b st'"
+      and frame: "frame_weak (TXY st',SY st', TYX st' - {b}, SX st' \<union> {b}) (TXY st, SY st, TYX st, SX st)"
+      and owns: "b \<in> TYX st'"
+    shows "I1 st K"
+  using assms subst unfolding frame_weak.simps I1_def
+    by (smt CleanQ_Set_Invariants_def I1_def Un_insert_right insert_Diff 
+          sup_aci(3) sup_assoc sup_bot.comm_neutral)
+
+lemma CleanQ_Set_deq_y_weak_I1:
+  fixes st st' K b
+  assumes I: "CleanQ_Set_Invariants K st'"
+      and rb: "st = CleanQ_Set_enq_y b st'"
+      and frame: "frame_weak (TYX st',SX st', TXY st' - {b}, SY st' \<union> {b}) (TYX st, SX st, TXY st, SY st)"
+      and owns: "b \<in> TXY st'"
+    shows "I1 st K"
+  using assms subst unfolding frame_weak.simps I1_def
+  by (smt CleanQ_Set_Invariants_def I1_def Un_insert_right insert_Diff 
+          sup_aci(3) sup_assoc sup_bot.comm_neutral)
+
+lemma CleanQ_Set_deq_x_weak_I2:
+  fixes st st' K b
+  assumes I: "CleanQ_Set_Invariants K st'"
+      and rb: "st = CleanQ_Set_enq_x b st'"
+      and frame: "frame_weak (TXY st',SY st', TYX st' - {b}, SX st' \<union> {b}) (TXY st, SY st, TYX st, SX st)"
+      and owns: "b \<in> TYX st'"
+    shows "I2 st"
+proof(unfold I2_def, intro conjI)
+  from frame obtain \<Delta>AB \<Delta>BC where
+    fA: "TXY st' = \<Delta>AB \<union> TXY st" and
+    fB: "SY st' \<union> \<Delta>AB = \<Delta>BC \<union> SY st" and
+    fC: "(TYX st' - {b}) \<union> \<Delta>BC = TYX st" and
+    fD: "SX st' \<union> {b} = SX st" and
+    dAB: "TXY st \<inter> \<Delta>AB = {}" and
+    dAC: "TXY st \<inter> \<Delta>BC = {}" and
+    dBC: "SY st \<inter> \<Delta>BC = {}"
+    by (metis (no_types, lifting) frame_weak.simps sup.commute)
+
+  from fA have ss_\<Delta>AB: "\<Delta>AB \<subseteq> TXY st'" by(auto)
+  with fB have ss_\<Delta>BC: "\<Delta>BC \<subseteq> TXY st' \<union> SY st'" by(auto)
+
+  from fA have ss_A: "TXY st \<subseteq> TXY st'" by(auto)
+  from fB ss_\<Delta>AB have ss_B: "SY st \<subseteq> TXY st' \<union> SY st'" by(auto)
+  from fC ss_\<Delta>BC have ss_C: "TYX st \<subseteq> TXY st' \<union> SY st' \<union> (TYX st' - {b})" by(auto)
+
+  from I owns ss_A show "SX st \<inter> TXY st = {}" by(unfold fD[symmetric],  auto simp:CleanQ_Set_Invariants_simp)
+  from I owns ss_B show "SX st \<inter> SY st = {}" by(unfold fD[symmetric],  auto simp:CleanQ_Set_Invariants_simp)
+  from I owns ss_C show "SX st \<inter> TYX st = {}" by(unfold fD[symmetric],  auto simp:CleanQ_Set_Invariants_simp)
+
+  from fC have "SY st \<inter> TYX st = SY st \<inter> ((TYX st' - {b}) \<union> \<Delta>BC)" by(simp)
+  also have "... = (SY st \<inter> (TYX st' - {b})) \<union> (SY st \<inter> \<Delta>BC)" by(auto)
+  also {
+    from ss_B have "SY st \<inter> (TYX st' - {b}) \<subseteq> (TXY st' \<union> SY st') \<inter> TYX st'" by(auto)
+    also from I have "... = {}" by( auto simp:CleanQ_Set_Invariants_simp)
+    finally have "(SY st \<inter> (TYX st' - {b})) \<union> (SY st \<inter> \<Delta>BC) = SY st \<inter> \<Delta>BC" by(simp)
+  }
+  txt \<open>@{term "SY st \<inter> \<Delta>BC = {}"} is essential\<close>
+  finally have "SY st \<inter> TYX st = SY st \<inter> \<Delta>BC" .
+  with dBC show "SY st \<inter> TYX st = {}" by simp
+
+  from fC have "TXY st \<inter> TYX st = TXY st \<inter> ((TYX st' - {b}) \<union> \<Delta>BC)" by simp
+  also have "... = (TXY st \<inter> (TYX st' - {b})) \<union> (TXY st \<inter> \<Delta>BC)" by blast
+  also {
+    from ss_A have "TXY st \<inter> (TYX st' - {b}) \<subseteq> (TXY st' \<union> {b}) \<inter> (TYX st' - {b})" by(auto)
+    also from I have "... = {}" by( auto simp:CleanQ_Set_Invariants_simp)
+    finally have "(TXY st \<inter> (TYX st' - {b})) \<union> (TXY st \<inter> \<Delta>BC) = TXY st \<inter> \<Delta>BC" by(simp)
+  }
+  txt \<open>@{term "TXY st \<inter> \<Delta>BC = {}"} is essential\<close>
+  finally have "TXY st \<inter> TYX st = TXY st \<inter> \<Delta>BC" .
+  with dAC show "TXY st \<inter> TYX st = {}" by(simp)
+
+  from fB have "TXY st \<inter> (\<Delta>BC \<union> SY st) = TXY st \<inter> (SY st' \<union> \<Delta>AB)" by(simp)
+  also have "... = (TXY st \<inter> SY st') \<union> (TXY st \<inter> \<Delta>AB)" by(auto)
+  also {
+    from ss_A have "TXY st \<inter> SY st' \<subseteq> (TXY st' \<union> {b}) \<inter> SY st'" by(auto)
+    also from I owns have "... = {}" by( auto simp:CleanQ_Set_Invariants_simp)
+    finally have "(TXY st \<inter> SY st') \<union> (TXY st \<inter> \<Delta>AB) = TXY st \<inter> \<Delta>AB" by(simp)
+  }
+  txt \<open>@{term "TXY st \<inter> \<Delta>AB = {}"} is essential, given @{term "TXY st \<inter> \<Delta>BC = {}"}.\<close>
+  finally have "TXY st \<inter> (\<Delta>BC \<union> SY st) = TXY st \<inter> \<Delta>AB" .
+  with dAB show " SY st \<inter> TXY st = {}" by(auto)
+qed
+
+
+lemma CleanQ_Set_deq_y_weak_I2:
+  fixes st st' K b
+  assumes I: "CleanQ_Set_Invariants K st'"
+      and rb: "st = CleanQ_Set_enq_y b st'"
+      and frame: "frame_weak (TYX st',SX st', TXY st' - {b}, SY st' \<union> {b}) (TYX st, SX st, TXY st, SY st)"
+      and owns: "b \<in> TXY st'"
+    shows "I2 st"
+proof(unfold I2_def, intro conjI)
+  from frame obtain \<Delta>AB \<Delta>BC where
+    fA: "TYX st' = \<Delta>AB \<union> TYX st" and
+    fB: "SX st' \<union> \<Delta>AB = \<Delta>BC \<union> SX st" and
+    fC: "(TXY st' - {b}) \<union> \<Delta>BC = TXY st" and
+    fD: "SY st' \<union> {b} = SY st" and
+    dAB: "TYX st \<inter> \<Delta>AB = {}" and
+    dAC: "TYX st \<inter> \<Delta>BC = {}" and
+    dBC: "SX st \<inter> \<Delta>BC = {}"
+    by (metis (no_types, lifting) frame_weak.simps sup.commute)
+
+  from fA have ss_\<Delta>AB: "\<Delta>AB \<subseteq> TYX st'" by(auto)
+  with fB have ss_\<Delta>BC: "\<Delta>BC \<subseteq> TYX st' \<union> SX st'" by(auto)
+
+  from fA have ss_A: "TYX st \<subseteq> TYX st'" by(auto)
+  from fB ss_\<Delta>AB have ss_B: "SX st \<subseteq> TYX st' \<union> SX st'" by(auto)
+  from fC ss_\<Delta>BC have ss_C: "TXY st \<subseteq> TYX st' \<union> SX st' \<union> (TXY st' - {b})" by(auto)
+
+  from I owns ss_A show "SY st \<inter> TYX st = {}" by(unfold fD[symmetric], auto simp:CleanQ_Set_Invariants_simp)
+  from I owns ss_B show "SX st \<inter> SY st = {}" by(unfold fD[symmetric], auto simp:CleanQ_Set_Invariants_simp)
+  from I owns ss_C show "SY st \<inter> TXY st = {}" by(unfold fD[symmetric], auto simp:CleanQ_Set_Invariants_simp)
+
+  from fC have "SX st \<inter> TXY st = SX st \<inter> ((TXY st' - {b}) \<union> \<Delta>BC)" by(simp)
+  also have "... = (SX st \<inter> (TXY st' - {b})) \<union> (SX st \<inter> \<Delta>BC)" by(auto)
+  also {
+    from ss_B have "SX st \<inter> (TXY st' - {b}) \<subseteq> (TYX st' \<union> SX st') \<inter> TXY st'" by(auto)
+    also from I have "... = {}" by(auto simp:CleanQ_Set_Invariants_simp)
+    finally have "(SX st \<inter> (TXY st' - {b})) \<union> (SX st \<inter> \<Delta>BC) = SX st \<inter> \<Delta>BC" by(simp)
+  }
+  txt \<open>@{term "SX st \<inter> \<Delta>BC = {}"} is essential\<close>
+  finally have "SX st \<inter> TXY st = SX st \<inter> \<Delta>BC" .
+  with dBC show "SX st \<inter> TXY st = {}" by simp
+
+  from fC have "TYX st \<inter> TXY st = TYX st \<inter> ((TXY st' - {b}) \<union> \<Delta>BC)" by simp
+  also have "... = (TYX st \<inter> (TXY st' - {b})) \<union> (TYX st \<inter> \<Delta>BC)" by blast
+  also {
+    from ss_A have "TYX st \<inter> (TXY st' - {b}) \<subseteq> (TYX st' \<union> {b}) \<inter> (TXY st' - {b})" by(auto)
+    also from I have "... = {}" by(auto simp:CleanQ_Set_Invariants_simp)
+    finally have "(TYX st \<inter> (TXY st' - {b})) \<union> (TYX st \<inter> \<Delta>BC) = TYX st \<inter> \<Delta>BC" by(simp)
+  }
+  txt \<open>@{term "TYX st \<inter> \<Delta>BC = {}"} is essential\<close>
+  finally have "TYX st \<inter> TXY st = TYX st \<inter> \<Delta>BC" .
+  with dAC show "TXY st \<inter> TYX st = {}" by auto
+
+  from fB have "TYX st \<inter> (\<Delta>BC \<union> SX st) = TYX st \<inter> (SX st' \<union> \<Delta>AB)" by(simp)
+  also have "... = (TYX st \<inter> SX st') \<union> (TYX st \<inter> \<Delta>AB)" by(auto)
+  also {
+    from ss_A have "TYX st \<inter> SX st' \<subseteq> (TYX st' \<union> {b}) \<inter> SX st'" by(auto)
+    also from I owns have "... = {}" by(auto simp:CleanQ_Set_Invariants_simp)
+    finally have "(TYX st \<inter> SX st') \<union> (TYX st \<inter> \<Delta>AB) = TYX st \<inter> \<Delta>AB" by(simp)
+  }
+  txt \<open>@{term "TYX st \<inter> \<Delta>AB = {}"} is essential, given @{term "TYX st \<inter> \<Delta>BC = {}"}.\<close>
+  finally have "TYX st \<inter> (\<Delta>BC \<union> SX st) = TYX st \<inter> \<Delta>AB" .
+  with dAB show " SX st \<inter> TYX st = {}" by(auto)
+qed
+
+
+
+lemma CleanQ_Set_deq_x_weak_Invariants :
+  fixes st st' K b
+  assumes I: "CleanQ_Set_Invariants K st'"
+      and rb: "st = CleanQ_Set_deq_x b st'"
+      and frame: "frame_weak (TXY st' ,SY st', TYX st' - {b}, SX st' \<union> {b}) (TXY st, SY st, TYX st, SX st)"
+      and owns: "b \<in> TYX st'"
+    shows "CleanQ_Set_Invariants K (CleanQ_Set_deq_x b st)"  
+  by (metis CleanQ_Set_State.select_convs(2) CleanQ_Set_State.select_convs(3) 
+      CleanQ_Set_State.select_convs(4) CleanQ_Set_deq_x_Invariants CleanQ_Set_deq_x_upd Diff_idemp I 
+      frame frame_weak.simps owns rb sup.right_idem)
+
+
+
+lemma CleanQ_Set_deq_y_weak_Invariants :
+  fixes st st' K b
+  assumes I: "CleanQ_Set_Invariants K st'"
+      and rb: "st = CleanQ_Set_deq_y b st'"
+      and frame: "frame_weak (TYX st' ,SX st', TXY st' - {b}, SY st' \<union> {b}) (TYX st, SX st, TXY st, SY st)"
+      and owns: "b \<in> TXY st'"
+    shows "CleanQ_Set_Invariants K (CleanQ_Set_deq_y b st)"   
+  by (metis CleanQ_Set_State.select_convs(1) CleanQ_Set_State.select_convs(3) 
+      CleanQ_Set_State.select_convs(4) CleanQ_Set_deq_y_Invariants CleanQ_Set_deq_y_upd Diff_idemp I 
+      frame frame_weak.simps owns rb sup.right_idem)
 
 (* ==================================================================================== *)
 subsection \<open>Integration in COMPLEX\<close>
